@prefix aowm:    <http://dqm.faw.jku.at/ontologies/aowm#> .
@prefix rdf:     <http://www.w3.org/1999/02/22-rdf-syntax-ns#> .
@prefix rdfs:    <http://www.w3.org/2000/01/rdf-schema#> .
@prefix owl:     <http://www.w3.org/2002/07/owl#> .
@prefix xsd:     <http://www.w3.org/2001/XMLSchema#> .
@prefix dct:     <http://purl.org/dc/terms/> .
@prefix dcterms: <http://purl.org/dc/terms/> .
@prefix dc:      <http://purl.org/dc/elements/1.1/> .
@prefix dcmi:    <http://purl.org/dc/dcmitype/> .
@prefix vann:    <https://vocab.org/vann/> .
@prefix foaf:    <http://xmlns.com/foaf/0.1/> .
@prefix prov:    <http://www.w3.org/ns/prov#> .
@prefix mod:     <https://w3id.org/mod#> .
@prefix bibo:    <http://purl.org/ontology/bibo/> .
@prefix schema:  <https://schema.org/> .
@prefix voaf:    <http://purl.org/vocommons/voaf#> .
@prefix idot:    <http://identifiers.org/idot/> .
@prefix omv:     <http://omv.ontoware.org/2005/05/ontology#> .
@prefix cc:      <http://creativecommons.org/ns#> .
@prefix odrl:    <http://www.w3.org/ns/odrl/2/> .
@prefix sd:      <http://www.w3.org/ns/sparql-service-description#> .
@prefix door:    <http://kannel.open.ac.uk/ontology#> .
@prefix pav:     <http://purl.org/pav/> .
@prefix xml:     <http://www.w3.org/XML/1998/namespace/> .
@prefix adms:    <http://www.w3.org/ns/adms#> .
@prefix dcat:    <http://www.w3.org/ns/dcat#> .
@prefix doap:    <http://usefulinc.com/ns/doap#> .
@prefix nkos:    <http://w3id.org/nkos#> .
@prefix sioc:    <http://rdfs.org/sioc/> .
@prefix skos:    <http://www.w3.org/2004/02/skos/core#> .
@prefix void:    <http://rdfs.org/ns/void#> .
@prefix frbr:    <http://purl.org/vocab/frbr/core#> .
@prefix oboinowl:<http://www.geneontology.org/formats/oboInOwl#> .
@prefix vcard:   <http://www.w3.org/2006/vcard/ns#> .

#################################################################
# Ontology Header 
#################################################################
<http://dqm.faw.jku.at/ontologies/aowm>
    a owl:Ontology ;
    dct:title "Vocabulary For Annotating Ontologies With Metadata"@en ;
    dct:creator "Moritz Haider" ;
    dct:description "A vocabulary designed to describe metadata about ontologies."@en ;
    dct:created "2026-01-31"^^xsd:date ;
    dct:license <http://creativecommons.org/licenses/by/4.0/> ;
    vann:preferredNamespacePrefix "aowm" ;
    vann:preferredNamespaceUri <http://dqm.faw.jku.at/ontologies/aowm#> ;
    owl:versionInfo "0.1" ;
    .   
#################################################################
# Classes 
#################################################################
aowm:Resource
    a owl:Class ;
	rdfs:subClassOf owl:Thing ;
    rdfs:label "Resource"@en ;
    rdfs:comment "Generic parent element for all domain classes in the AOWM vocabulary. Used as the common superclass for ontology metadata resources (Elements, Version, ...)."@en ;
    rdfs:isDefinedBy <http://dqm.faw.jku.at/ontologies/aowm> ;
	dct:issued "2026-01-31"^^xsd:date .
	
aowm:Ontology
    a owl:Class ;
	rdfs:subClassOf aowm:Resource, mod:SemanticArtefact, owl:Ontology ;
    rdfs:label "Ontology"@en ;
    rdfs:comment "A formal specification of a conceptualization, described using RDF-based standards."@en ;
    rdfs:isDefinedBy <http://dqm.faw.jku.at/ontologies/aowm> ;
	dct:issued "2026-01-31"^^xsd:date ;
	rdfs:seeAlso owl:Ontology .
	
aowm:Distribution
    a owl:Class ;
	rdfs:subClassOf aowm:Resource, mod:SemanticArtefactDistribution ;
    rdfs:label "Distribution of an ontology"@en ;
    rdfs:comment "A specific representation and/or serialization of an ontology."@en ;
    rdfs:isDefinedBy <http://dqm.faw.jku.at/ontologies/aowm> ;
	dct:issued "2026-01-31"^^xsd:date .

aowm:Catalog
    a owl:Class ;
	rdfs:subClassOf aowm:Resource, mod:SemanticArtefactCatalog ;
    rdfs:label "Data Catalog"@en ;
    rdfs:comment "A dedicated web-based system that fosters the availability, discoverability and long-term preservation and maintenance of semantic artefacts, including ontologies."@en ;
    rdfs:isDefinedBy <http://dqm.faw.jku.at/ontologies/aowm> ;
	dct:issued "2026-01-31"^^xsd:date .
	
aowm:CatalogRecord
    a owl:Class ;
	rdfs:subClassOf aowm:Resource, mod:SemanticArtefactCatalogRecord ;
    rdfs:label "Ontology Data Catalog Record"@en ;
    rdfs:comment "A record in a catalog, describing the registration of a single ontology."@en ;
    rdfs:isDefinedBy <http://dqm.faw.jku.at/ontologies/aowm> ;
	dct:issued "2026-01-31"^^xsd:date .
	
aowm:Version
    a owl:Class ;
    rdfs:subClassOf aowm:Resource ;
    rdfs:label "Version"@en ;
    rdfs:comment "A specific version of an ontology or metadata record."@en ;
	rdfs:seeAlso mod:SemanticArtefactVersion ;
	dct:issued "2026-01-31"^^xsd:date .
	
aowm:Agent
    a owl:Class ;
	rdfs:subClassOf aowm:Resource, foaf:Agent ;
    rdfs:label "Agent"@en ;
    rdfs:isDefinedBy <http://dqm.faw.jku.at/ontologies/aowm> ;
	rdfs:comment "A resource that acts or has the power to act."@en ;
	dct:issued "2026-01-31"^^xsd:date .
	
aowm:Role
	a owl:Class ;
	rdfs:label "Role"@en ;
    rdfs:comment "A role assumed by an agent in relation to a resource."@en ;
    rdfs:isDefinedBy <http://dqm.faw.jku.at/ontologies/aowm> ;
	dct:issued "2026-01-31"^^xsd:date ;
	rdfs:seeAlso prov:Role .
	
aowm:Person
    a owl:Class ;
	rdfs:subClassOf aowm:Agent ;
	rdfs:label "Person"@en ;
	rdfs:isDefinedBy <http://dqm.faw.jku.at/ontologies/aowm> ;
	dct:issued "2026-01-31"^^xsd:date ;
	rdfs:seeAlso foaf:Person .

aowm:Organization
    a owl:Class ;
	rdfs:subClassOf aowm:Agent ;
	rdfs:label "Organization"@en ;
	rdfs:isDefinedBy <http://dqm.faw.jku.at/ontologies/aowm> ;
	dct:issued "2026-01-31"^^xsd:date ;
	rdfs:seeAlso foaf:Organization .
	
aowm:SerializationFormat
    a owl:Class ;
	rdfs:subClassOf aowm:Resource ;
    rdfs:label "Serialization Format"@en ;
	rdfs:isDefinedBy <http://dqm.faw.jku.at/ontologies/aowm> ;
	dct:issued "2026-01-31"^^xsd:date .
	
aowm:DegreeOfMaturity
	a owl:Class ;
	rdfs:subClassOf aowm:Resource ;
    rdfs:label "Degree Of Maturity"@en ;
    rdfs:isDefinedBy <http://dqm.faw.jku.at/ontologies/aowm> ;
	dct:issued "2026-01-31"^^xsd:date .
	
aowm:MetadataCreationMethod
	a owl:Class ;
	rdfs:subClassOf aowm:Resource ;
    rdfs:label "Creation Method Of Metadata"@en ;
	rdfs:isDefinedBy <http://dqm.faw.jku.at/ontologies/aowm> ;
	dct:issued "2026-01-31"^^xsd:date .
	
#################################################################
#Concepts 
#################################################################	
aowm:DegreeOfMaturityScheme
    a skos:ConceptScheme ;
    rdfs:label "Degree of Maturity Scheme"@en ;
    skos:hasTopConcept aowm:Draft, aowm:Stable, aowm:Mature ;
    dct:isPartOf <http://dqm.faw.jku.at/ontologies/aowm> ;
	dct:issued "2026-01-31"^^xsd:date .
	
aowm:Draft
    a aowm:DegreeOfMaturity, skos:Concept ;
    rdfs:label "Draft"@en ;
    skos:inScheme aowm:DegreeOfMaturityScheme ;
    skos:definition "Ontology is in early development stage; incomplete and experimental."@en .

aowm:Stable
    a aowm:DegreeOfMaturity, skos:Concept ;
    rdfs:label "Stable"@en ;
    skos:inScheme aowm:DegreeOfMaturityScheme ;
    skos:definition "Ontology is stable, can be used for production, minor changes expected."@en .

aowm:Mature
    a aowm:DegreeOfMaturity, skos:Concept ;
    rdfs:label "Mature"@en ;
    skos:inScheme aowm:DegreeOfMaturityScheme ;
    skos:definition "Ontology is fully mature, stable, widely adopted, unlikely to change."@en .
	
aowm:SerializationFormatScheme
    a skos:ConceptScheme ;
    skos:hasTopConcept aowm:Turtle, aowm:RdfXml, aowm:JsonLd, aowm:NTriples, aowm:Trig ;
    rdfs:label "Serialization Format Scheme"@en ;
	dct:isPartOf <http://dqm.faw.jku.at/ontologies/aowm> ;
	dct:issued "2026-01-31"^^xsd:date .
	
aowm:Turtle
    a aowm:SerializationFormat, skos:Concept ;
    rdfs:label "Turtle"@en ;
    skos:inScheme aowm:SerializationFormatScheme ;
    skos:definition "Serialization with Turtle."@en .
	
aowm:RdfXml
    a aowm:SerializationFormat, skos:Concept ;
    rdfs:label "RDF/XML"@en ;
    skos:inScheme aowm:SerializationFormatScheme ;
    skos:definition "Serialization with RDF/XML"@en .
	
aowm:JsonLd
    a aowm:SerializationFormat, skos:Concept ;
    rdfs:label "JSON-LD"@en ;
    skos:inScheme aowm:SerializationFormatScheme ;
    skos:definition "Serialization with JSON-LD"@en .
	
aowm:NTriples
    a aowm:SerializationFormat, skos:Concept ;
    rdfs:label " N-Triples"@en ;
    skos:inScheme aowm:SerializationFormatScheme ;
    skos:definition "Serialization with N-Triples"@en .
	
aowm:Trig
    a aowm:SerializationFormat, skos:Concept ;
    rdfs:label "TriG"@en ;
    skos:inScheme aowm:SerializationFormatScheme ;
    skos:definition "Serialization with TriG"@en .
	
aowm:MetadataCreationMethodScheme
    a skos:ConceptScheme ;
    skos:hasTopConcept aowm:Manual, aowm:Automatic, aowm:SemiAutomatic ;
    rdfs:label "Metadata Creation Method Scheme"@en ;
	dct:isPartOf <http://dqm.faw.jku.at/ontologies/aowm> ;
	dct:issued "2026-01-31"^^xsd:date .
	
aowm:Manual
    a aowm:MetadataCreationMethod, skos:Concept ;
    rdfs:label "Manual"@en ;
    skos:inScheme aowm:MetadataCreationMethodScheme ;
    skos:definition "Manual metadata creation"@en .

aowm:Automatic
    a aowm:MetadataCreationMethod, skos:Concept ;
    rdfs:label "Automatic"@en ;
    skos:inScheme aowm:MetadataCreationMethodScheme ;
    skos:definition "Automatic metadata creation"@en .
	
aowm:SemiAutomatic
    a aowm:MetadataCreationMethod, skos:Concept ;
    rdfs:label "Semi-Automatic"@en ;
    skos:inScheme aowm:MetadataCreationMethodScheme ;
    skos:definition "Semi-Automatic metadata creation"@en .
	
#################################################################
#Properties 
#################################################################
####General properties####
dct:title
    rdf:type rdf:Property ;
    rdfs:label "title"@en ;
	dct:domainIncludes  
		aowm:Ontology ,
        aowm:Distribution,
		aowm:Catalog ;
    dct:description  "dct: A name given to the resource. OMV: The name by which an ontology is formally known. RDFS: A human-readable name for the subject. FOAF:  A name for some thing. SKOS: The preferred and alternative labels are useful when generating or creating human-readable representations of a knowledge organization system. SCHEMA: The name of the item."@en ;
	rdfs:isDefinedBy <http://purl.org/dc/terms/> ;	
	dct:issued "2008-01-14"^^xsd:date ;
	owl:equivalentProperty  
		rdfs:label ,
        cc:attributionName ,
        omv:name ,
        schema:name ,
        skos:prefLabel ,
        foaf:name .
		
### https://w3id.org/mod#acronym
mod:acronym
    a owl:DatatypeProperty ;
	rdfs:subPropertyOf mod:acronym ;
    rdfs:label "acronym"@en ;
	rdfs:domain mod:SemanticArtefact ;
	dct:domainIncludes aowm:Ontology ;
	rdfs:range xsd:string ;
    dct:description     "MOD: Short acronym label, often used as an identifier within some ontology platforms such as BioPortal or OBO Foundry. OMV: A short name by which an ontology is formally known."@en ;
     rdfs:isDefinedBy        <http://omv.ontoware.org/2005/05/ontology> ;
     dct:issued          "2009-12-24"^^xsd:date .
	 
	 
### https://w3id.org/mod#URI
mod:URI             rdf:type                owl:DatatypeProperty ;
                    rdfs:label              "URI"@en ;
                    rdfs:domain             mod:SemanticArtefact ;
					dct:domainIncludes 		aowm:Ontology ;
                    rdfs:range              xsd:anyURI ;
                    dct:description     "OMV: The URI of the ontology which is described by this metadata."@en ;
                    rdfs:isDefinedBy        <http://omv.ontoware.org/2005/05/ontology> ;
                    dct:issued          "2009-12-24"^^xsd:date ;
                    owl:equivalentProperty  omv:URI . 
	
### http://purl.org/dc/terms/identifier                 
dct:identifier  
	rdf:type rdf:Property ;
    rdfs:subPropertyOf dc:identifier  ;
    rdfs:label "other identifier"@en ;
    dct:domainIncludes  aowm:Ontology ,
						aowm:Catalog ;
	rdfs:range rdfs:Literal ;
    dct:description     "dct: An unambiguous reference to the resource within a given context. Recommended practice is to identify the resource by means of a string conforming to an identification system. Examples include International Standard Book Number (ISBN), Digital Object Identifier (DOI), and Uniform Resource Name (URN).  Persistent identifiers should be provided as HTTP URIs. SKOS: A notation is a string of characters such as 'T58.5' or '303.4833' used to uniquely identify a concept within the scope of a given concept scheme. ADMS: adms:identifier is used to link any resource to an instance of adms:Identifier which is its range. N.B. it is not appropriate to use dct:identifer to link to the Identifier class as its range is rdfs:Literal. ADMS uses this to provide any identifier for the Asset. SCHEMA: The identifier property represents any kind of identifier for any kind of Thing, such as ISBNs, GTIN codes, UUIDs etc. Schema.org provides dedicated properties for representing many of these, either as textual strings or as URL (URI) links. DCAT: A unique identifier of the item."@en ;
    rdfs:isDefinedBy <http://purl.org/dc/terms/> ;
    dct:issued "2008-01-14"^^xsd:date ;
    owl:equivalentProperty  
		skos:notation ,
        schema:identifier .
		
### https://w3id.org/mod#hasRepresentationLanguage
mod:has
	rdf:tpye owl:DatatypeProperty ;
	rdfs:label "representation language."@en ;
	rdfs:subPropertyOf mod:hasRepresentationLangauge ;
	rdfs:domain mod:SemanticArtefactDistribution ;
	dct:domainIncludes aowm:Distribution ;
	rdfs:range xsd:string ;
	dct:description "MOD: A language that is used to create an ontology. OMV: The ontology language."@en ;
	rdfs:isDefinedBy <http://dqm.faw.jku.at/ontologies/aowm> ;
	dct:issued          "2009-12-24"^^xsd:date ;
	owl:equivalentProperty  omv:hasOntologyLanguage , schema:fileFormat .
	
### https://w3id.org/mod#hasFormalityLevel
mod:hasFormalityLevel
	rdf:tpye owl:DatatypeProperty ;
	rdfs:label "formality level."@en ;
	rdfs:subPropertyOf mod:hasFormalityLevel ;
	rdfs:domain             mod:SemanticArtefact ;	
	dct:domainIncludes		aowm:Ontology ;
	rdfs:range xsd:string ;
	dct:description     "MOD: The level of formality of an ontology. OMV: Level of formality of the ontology."@en ;
	rdfs:isDefinedBy <http://dqm.faw.jku.at/ontologies/aowm> ;
	dct:issued "2025-11-20"^^xsd:date ;
	owl:equivalentProperty omv:hasFormalityLevel, schema:fileFormat .

### https://w3id.org/mod#hasSyntax
mod:hasSyntax
	rdf:tpye owl:DatatypeProperty ;
	rdfs:label "syntax."@en ;
	rdfs:subPropertyOf mod:hasSyntax ;
	rdfs:domain mod:SemanticArtefactDistribution ;
	dct:domainIncludes aowm:Distribution ;
	rdfs:range xsd:anyURI ;
    dct:description     "MOD: The syntax followed in the creation of an ontology. OMV: The presentation syntax for the ontology langage."@en ;
	rdfs:isDefinedBy <http://dqm.faw.jku.at/ontologies/aowm> ;
	 dct:issued          "2009-12-24"^^xsd:date ;
	owl:equivalentProperty omv:hasOntologySyntax, dct:format .
	
### http://purl.org/dc/terms/language
dct:language    
	rdf:type rdf:Property ;
    rdfs:subPropertyOf dc:language ;
    rdfs:label "natural language"@en ;
    dct:domainIncludes aowm:Ontology, aowm:Catalog ;
    dct:description     "dct: A language of the resource. Recommended practice is to use either a non-literal value representing a language from a controlled vocabulary such as ISO 639-2 or ISO 639-3, or a literal value consisting of an IETF Best Current Practice 47 [[IETF-BCP47](https://tools.ietf.org/html/bcp47)] language tag. OMV: The language of the content of the ontology, i.e. English, French, etc. DOAP: ISO language code a project has been translated into."@en ;
    rdfs:isDefinedBy <http://purl.org/dc/terms/> ;
    dct:issued          "2008-01-14"^^xsd:date ;
    owl:equivalentProperty  omv:naturalLanguage, schema:inLanguage, doap:language .
	
### http://purl.org/dc/terms/type
dct:type        
	rdf:type rdf:Property ;
    rdfs:subPropertyOf dc:type ;
    rdfs:label"generic type"@en ;
    dct:domainIncludes aowm:Ontology, aowm:Catalog ;
     dct:description     "dct: The nature or genre of the resource. Recommended practice is to use a controlled vocabulary such as the DCMI Type Vocabulary [[DCMI-TYPE](http://dublincore.org/documents/dcmi-type-vocabulary/)]. To describe the file format, physical medium, or dimensions of the resource, use the property Format. OMV: The nature of the content of the ontology."@en ;
    rdfs:isDefinedBy <http://purl.org/dc/terms/> ;
     dct:issued          "2008-01-14"^^xsd:date ;
    owl:equivalentProperty omv:isOfType .
	
aowm:doi
	a owl:DatatypeProperty ;
	rdfs:subPropertyOf bibo:doi ;
	rdfs:domain aowm:Ontology ;
	rdfs:range xsd:string ;
	rdfs:label "DOI"@en ;
	dct:description "Specifies the DOI for citing the ontology."@en ;
    rdfs:isDefinedBy <http://dqm.faw.jku.at/ontologies/aowm> .
	
aowm:bibliographicCitation
	a owl:DatatypeProperty ;
	rdfs:subPropertyOf bibo:doi ;
	rdfs:domain aowm:Ontology ;
	rdfs:range xsd:string ;
	rdfs:label "Bibliographic Citation"@en ;
	dct:description "Bibliographic Citation."@en ;
    rdfs:isDefinedBy <http://dqm.faw.jku.at/ontologies/aowm> .
								
#### license properties ####
### http://purl.org/dc/terms/accessRights
dct:accessRights
    rdf:type rdf:Property ;
    rdfs:subPropertyOf dc:rights , dct:rights ;
    rdfs:label "access rights"@en ;
    dct:domainIncludes aowm:Ontology, aowm:Catalog ;
    dct:description     "dct: Information about who access the resource or an indication of its security status. Access Rights may include information regarding access or restrictions based on privacy, security, or other policies. MOD: Information on access (i.e., read, download) to an ontology."@en ;
    rdfs:isDefinedBy <http://purl.org/dc/terms/> ;
     dct:issued          "2003-02-15"^^xsd:date .

### http://purl.org/dc/terms/license
dct:license     
	rdf:type rdf:Property ;
    rdfs:subPropertyOf dc:rights, dct:rights ;
	rdfs:label "license"@en ;
    dct:domainIncludes aowm:Ontology, aowm:Catalog ;
    dct:description     "dct: A legal document giving official permission to do something with the resource. Recommended practice is to identify the license document with a URI. If this is not possible or feasible, a literal value that identifies the license may be provided. dct:rights Information about rights held in and over the resource. OMV: Underlying license model. SCHEMA: A license document that applies to this content, typically indicated by URL."@en ;
    rdfs:isDefinedBy <http://purl.org/dc/terms/> ;
	dct:issued          "2004-06-14"^^xsd:date ;
    owl:equivalentProperty  cc:license, omv:license, schema:license .
        
### http://creativecommons.org/ns#useGuidelines
cc:useGuidelines     
	rdf:type rdf:Property ;
    rdfs:subPropertyOf dct:relation ;
	rdfs:label "use guidelines"@en ;
	rdfs:domain cc:Work ;
	rdfs:range rdfs:Resource ;
    dct:domainIncludes aowm:Ontology, aowm:Catalog, aowm:Distribution ;
    dct:description     "CC: A related resource which defines non-binding use guidelines for the work."@en ;     
	rdfs:isDefinedBy <http://purl.org/dc/terms/> ;
	 dct:issued          "2008-03-03"^^xsd:date ;
    owl:equivalentProperty  cc:license, omv:license, schema:license .
   
 ### http://creativecommons.org/ns#morePermissions
cc:morePermissions  
	rdf:type rdf:Property ;
    rdfs:subPropertyOf dct:relation ; 
    rdfs:label "more permissions"@en ;
    rdfs:domain cc:Work ;
    dct:domainIncludes aowm:Ontology, aowm:Catalog ;
    rdfs:range rdfs:Resource ;
                    dct:description     "CC: A related resource which describes additional permissions or alternative licenses for a Work which may be available."@en ;     
    rdfs:isDefinedBy <http://creativecommons.org/ns#> ;
	dct:issued          "2008-03-03"^^xsd:date .
	
### http://purl.org/dc/terms/rightsHolder
dct:rightsHolder  
	rdf:type rdf:Property ;
    rdfs:subPropertyOf dct:relation ; 
    rdfs:label "rights holder"@en ;
    dct:domainIncludes aowm:Ontology, aowm:Catalog ;
                    dct:description     "dct: A person or organization owning or managing rights over the resource. MOD: The person who can be contacted to enquire about an ontology. SCHEMA: The party holding the legal copyright to the CreativeWork. DCAT: Relevant contact information for the cataloged resource. Use of vCard is recommended."@en ;
    rdfs:isDefinedBy <http://purl.org/dc/terms/> ;
	owl:equivalentProperty  schema:copyrightHolder ;
	 dct:issued          "2004-06-14"^^xsd:date .

#### http://www.w3.org/ns/odrl/2/hasPolicy
odrl:hasPolicy 
	rdf:type rdf:Property, owl:ObjectProperty ;
    rdfs:label "target policy"@en ;
	rdfs:domain odrl:Asset ;
	rdfs:range odrl:Policy ;
    dct:domainIncludes aowm:Ontology, aowm:Catalog ;
                   dct:description      "ORDL: Identifies an ODRL Policy for which the identified Asset is the target Asset to all the Rules. DCAT: An ODRL conformant policy expressing the rights associated with the resource."@en ;
    rdfs:isDefinedBy <http://www.w3.org/ns/odrl/2/> ;
	dct:issued           "2018-02-15"^^xsd:date  .
	
####description properties####
dct:description rdf:type                rdf:Property ;
                    rdfs:subPropertyOf      dc:description ;
                    rdfs:label              "description"@en ;
                    dct:domainIncludes  aowm:Ontology ,
                                            aowm:Distribution ,
                                            aowm:Catalog ;
                    dct:description     "An account of the resource. Description may include but is not limited to: an abstract, a table of contents, a graphical representation, or a free-text account of the resource."@en ;
                    rdfs:isDefinedBy        <http://purl.org/dc/terms/> ;
                    dct:issued          "2008-01-14"^^xsd:date ;
                    owl:equivalentProperty  omv:description ,
                                            schema:description ,
                                            doap:description .
            
### http://xmlns.com/foaf/0.1/homepage
foaf:homepage       rdf:type                rdf:Property , owl:InverseFunctionalProperty , owl:ObjectProperty  ;
                    rdfs:subPropertyOf      foaf:page , foaf:isPrimaryTopicOf ;
                    rdfs:label              "homepage"@en ;
                    rdfs:domain             owl:Thing ;
                    dct:domainIncludes  	aowm:Ontology ,
                                            aowm:Catalog ,
                                            aowm:CatalogRecord ;
                    rdfs:range              foaf:Document ;
                    dct:description     "FOAF: A homepage for some thing."@en ;
                    rdfs:isDefinedBy        <http://xmlns.com/foaf/0.1/> ;
                     dct:issued          "2014-01-14"^^xsd:date ;
                    owl:equivalentProperty  schema:mainEntityOfPage ,
                                            cc:attributionURL ,
                                            doap:blog .
											
### http://www.w3.org/ns/dcat#landingPage
dcat:landingPage    rdf:type                rdf:Property , owl:ObjectProperty ;
                    rdfs:subPropertyOf      foaf:page ; 
                    rdfs:label              "documentation"@en ;
                    dct:domainIncludes  aowm:Ontology ,
                                            aowm:Catalog ;
                    rdfs:range              foaf:Document ;
                    dct:description     "DCAT: A Web page that can be navigated to in a Web browser to gain access to the dataset, its distributions and/or additional information. MOD: A link to the documentation page on a thing. OMV: URL for further documentation. RDFS: Further information about the subject resource. DOAP: URL of Wiki for collaborative discussion of project. VANN: A reference to a resource that provides information on how this resource is to be used. SCHEMA: Further documentation describing the Web API in more detail."@en ;
                    rdfs:isDefinedBy        <http://www.w3.org/TR/vocab-dcat/> ;
                    dct:issued          "2014-01-16"^^xsd:date ;
                    owl:equivalentProperty  omv:documentation ,
                                            vann:usageNote ,
                                            doap:wiki ,
                                            rdfs:seeAlso ,
                                            schema:documentation ,
                                            <http://www.isibang.ac.in/ns/mod/1.0/document> .	

### http://schema.org/featureList
schema:featureList  rdf:type                rdf:Property ;
                    rdfs:label              "feature list"@en ;
                    dct:domainIncludes  aowm:Catalog  ;
                    dct:description     "SCHEMA: Features or modules provided by this application (and possibly required by other applications)."@en ;
                    rdfs:isDefinedBy        <http://schema.org/> ;
                    dct:issued          "2012-04-21"^^xsd:date .		
			
### http://www.w3.org/2000/01/rdf-schema#comment
rdfs:comment        rdf:type                rdf:Property ;
                    rdfs:label              "notes or comments"@en ;
                    rdfs:domain             rdfs:Resource ;
                    dct:domainIncludes  aowm:Ontology ,
                                            aowm:Catalog ;
                    rdfs:range              rdfs:Literal ;           
                    dct:description     "RDFS: A description of the subject resource. OMV: Additional information about the ontology that is not included somewhere else (e.g. information that you do not want to include in the documentation). ADMS: A description of changes between this version and the previous version of the Asset."@en ;
                    rdfs:isDefinedBy        <http://www.w3.org/2000/01/rdf-schema#> ;
                    dct:issued          "2002-04-30"^^xsd:date ;
                    owl:equivalentProperty  omv:notes ,
                                            dct:description ,
                                            adms:versionNotes .			
			
### http://www.w3.org/ns/dcat#keyword
dcat:keyword        rdf:type                rdf:Property , owl:DatatypeProperty ;
                    rdfs:subPropertyOf      dct:subject ; 
                    rdfs:label              "keyword"@en ;
                    dct:domainIncludes  aowm:Ontology ,
                                            aowm:Catalog ;
                    rdfs:range              rdfs:Literal ;
                    dct:description     "DCAT: A keyword or tag describing a resource. MOD: A keyword(s) is used to describe the content of an ontology. OMV: List of keywords related to an ontology. SCHEMA: Keywords or tags used to describe this content. Multiple entries in a keywords list are typically delimited by commas."@en ;
                    rdfs:isDefinedBy        <http://www.w3.org/TR/vocab-dcat/> ;
                    dct:issued          "2014-01-16"^^xsd:date ;
                    owl:equivalentProperty   omv:keywords ,
                                             schema:keywords ,
                                             <http://www.isibang.ac.in/ns/mod/1.1/keyword> .		
### http://purl.org/dc/terms/alternative
dct:alternative rdf:type                rdf:Property ;
                    rdfs:subPropertyOf      dc:title , dct:title ;
                    rdfs:label              "alternative name"@en ;
                    dct:domainIncludes  aowm:Ontology ,
                                            aowm:Catalog ;
                    rdfs:range              rdfs:Literal ;
                    dct:description     "dct: An alternative name for the resource. The distinction between titles and alternative titles is application-specific. SKOS: The preferred and alternative labels are useful when generating or creating human-readable representations of a knowledge organization system. SCHEMA: An alias for the item. A short label that is used by some communities to refer to a dataset (see 'preferredPrefix')."@en ;
                    rdfs:isDefinedBy        <http://purl.org/dc/terms/> ;
                    dct:issued          "2000-07-11"^^xsd:date ;
                    owl:equivalentProperty  idot:alternatePrefix ,
                                            schema:alternateName ,
                                            skos:altLabel .
### http://www.w3.org/2004/02/skos/core#hiddenLabel
skos:hiddenLabel    rdf:type                rdfs:Property ,
                                            owl:AnnotationProperty ;
                    rdfs:subPropertyOf      rdfs:label ;
                    rdfs:label              "hidden label"@en ;
                    dct:domainIncludes  aowm:Ontology ,
                                            aowm:Catalog ;
                    rdfs:range              rdfs:Literal ;
                    dct:description     "MOD: Hidden or past name. SKOS: A lexical label for a resource that should be hidden when generating visual displays of the resource, but should still be accessible to free text search operations."@en;
                    rdfs:isDefinedBy        <http://www.w3.org/2004/02/skos/core> ;
                    dct:issued          "2009-08-18"^^xsd:date .
					
### http://purl.org/dc/terms/abstract
dct:abstract    rdf:type                rdf:Property ;
                    rdfs:subPropertyOf      dc:description , dct:description ;
                    rdfs:label              "abstract"@en ;
                    dct:domainIncludes  aowm:Ontology ,
                                            aowm:Catalog ;
                    dct:description     "dct: A summary of the resource."@en ;
                    rdfs:isDefinedBy        <http://purl.org/dc/terms/> ;
                    dct:issued          "2000-07-11"^^xsd:date .
            

### http://purl.org/dc/terms/bibliographicCitation
dct:bibliographicCitation
                    rdf:type                rdf:Property ;
                    rdfs:subPropertyOf      dc:identifier , dct:identifier ;
                    rdfs:label              "bibliographic reference"@en ;
                    dct:domainIncludes  aowm:Ontology ,
                                            aowm:Catalog ;
                    rdfs:range              rdfs:Literal ;
                    dct:description     "dct: A bibliographic reference for the resource. Recommended practice is to include sufficient bibliographic detail to identify the resource as unambiguously as possible. OMV: List of bibliographic references describing the ontology and its applications. FOAF: A document that this thing is the primary topic of"@en ;
                    rdfs:isDefinedBy        <http://purl.org/dc/terms/> ;
                    dct:issued          "2003-02-15"^^xsd:date .


### http://purl.org/dc/terms/isReferencedBy
dct:isReferencedBy
                    rdf:type                rdf:Property ;
                    rdfs:subPropertyOf      dc:relation , dct:relation ;
                    rdfs:label              "is referenced by"@en ;
                    dct:domainIncludes  aowm:Ontology ,
                                            aowm:Catalog ;
                    dct:description     "dct: A related resource that references, cites, or otherwise points to the described resource. DCAT: A related resource, such as a publication, that references, cites, or otherwise points to the cataloged resource."@en ;
                    rdfs:isDefinedBy        <http://purl.org/dc/terms/> ;
                    dct:issued          "2000-07-11"^^xsd:date .
					
####metrics#####
### https://w3id.org/mod#metrics
mod:metrics         rdf:type                owl:DatatypeProperty ;
                    rdfs:label              "metrics"@en ;
                    rdfs:domain             aowm:Ontology ,
                                            aowm:Distribution , 
                                            aowm:Catalog ;
                    rdfs:range              xsd:nonNegativeInteger ,
                                            xsd:decimal ;
                    dct:description     "MOD: A generic property to store any metrics (number) related to the ontology."@en ;
                    rdfs:isDefinedBy        <https://w3id.org/mod> ;
                    dct:issued          "2018-08-02"^^xsd:date .

###  https://w3id.org/mod#numberOfClasses
mod:numberOfClasses rdf:type                owl:DatatypeProperty ;
                    rdfs:subPropertyOf      mod:metrics ;
                    rdfs:label              "number of classes"@en ;
                    rdfs:domain             mod:SemanticArtefactDistribution ,
                                            mod:SemanticArtefactCatalog ;
					dct:domainIncludes		aowm:Distribution ,
											aowm:Catalog;
                    rdfs:range              xsd:nonNegativeInteger ;
                    dct:description     "MOD: The total number of classes in an ontology. OMV: Number of classes in the ontology. VOAF: The number of classes defined in the vocabulary namespace. Classes imported from other namespaces are not taken into account. VOID: The total number of distinct classes in a void:Dataset. In other words, the number of distinct resources occuring as objects of rdf:type."@en ;
                    rdfs:isDefinedBy        <http://omv.ontoware.org/2005/05/ontology> ;
                    dct:issued          "2009-12-24"^^xsd:date ;
                    owl:equivalentProperty  omv:numberOfClasses ,
                                            voaf:classNumber ,
                                            void:classes ,
                                            <http://www.isibang.ac.in/ns/mod/1.0/noOfClasses> .


###  https://w3id.org/mod#numberOfIndividuals
mod:numberOfIndividuals
                    rdf:type                owl:DatatypeProperty ;
                    rdfs:subPropertyOf      mod:metrics ;
                    rdfs:label              "number of individuals"@en ;
                    rdfs:domain             mod:SemanticArtefactDistribution ,
                                            mod:SemanticArtefactCatalog ;
					dct:domainIncludes	aowm:Distribution ,
											aowm:Catalog ;
                    rdfs:range              xsd:nonNegativeInteger ;
                    dct:description     "MOD: The total number of individuals in an ontology. OMV: Number of individuals in the ontology. VOID: The total number of entities that are described in a void:Dataset."@en ;
                    rdfs:isDefinedBy        <http://omv.ontoware.org/2005/05/ontology> ;
                    dct:issued          "2009-12-24"^^xsd:date ;
                    owl:equivalentProperty  omv:numberOfIndividuals ,
                                            void:entities ,
                                            <http://www.isibang.ac.in/ns/mod/1.0/noOfIndividuals> .


###  https://w3id.org/mod#numberOfProperties
mod:numberOfProperties
                    rdf:type                owl:DatatypeProperty ;
                    rdfs:subPropertyOf      mod:metrics ;
                    rdfs:label              "number of properties"@en ;
                    rdfs:domain             mod:SemanticArtefactDistribution ,
                                            mod:SemanticArtefactCatalog ;
					dct:domainIncludes	aowm:Distribution ,
											aowm:Catalog ;
                    rdfs:range              xsd:nonNegativeInteger ;
                    dct:description     "MOD: The total number of properties in an ontology. OMV: Number of properties in the ontology. VOAF: The number of properties defined in the vocabulary namespace. Properties imported from other namespaces are not taken into account. VOID: The total number of distinct properties in a void:Dataset. In other words, the number of distinct resources that occur in the predicate position of triples in the dataset."@en ;
                    rdfs:isDefinedBy        <http://omv.ontoware.org/2005/05/ontology> ;
                    dct:issued          "2009-12-24"^^xsd:date ;
                    owl:equivalentProperty  omv:numberOfProperties ,
                                            voaf:propertyNumber ,
                                            void:properties ,
                                            <http://www.isibang.ac.in/ns/mod/1.0/noOfProperties> .


###  https://w3id.org/mod#numberOfObjectProperties
mod:numberOfObjectProperties
                    rdf:type                owl:DatatypeProperty ;
                    rdfs:subPropertyOf      mod:numberOfProperties ;
                    rdfs:label              "number of object properties"@en ;
                    rdfs:domain             mod:SemanticArtefactDistribution ,
                                            mod:SemanticArtefactCatalog ;
					dct:domainIncludes	aowm:Distribution ,
											aowm:Catalog ;
                    rdfs:range              xsd:nonNegativeInteger ;
                    dct:description     "MOD: The total number of object properties in an ontology."@en ;
                    rdfs:isDefinedBy        <https://w3id.org/mod> ;
                    dct:issued          "2017-07-06"^^xsd:date .


###  https://w3id.org/mod#numberOfDataProperties
mod:numberOfDataProperties
                    rdf:type                owl:DatatypeProperty ;
                    rdfs:subPropertyOf      mod:numberOfProperties ;
                    rdfs:label              "number of data properties"@en ;
                    rdfs:domain             mod:SemanticArtefactDistribution ,
                                            mod:SemanticArtefactCatalog ;
					dct:domainIncludes	aowm:Distribution ,
											aowm:Catalog ;
                    rdfs:range              xsd:nonNegativeInteger ;
                    dct:description     "MOD: The total number of data properties in an ontology."@en ;
                    rdfs:isDefinedBy        <https://w3id.org/mod> ;
                    dct:issued          "2017-07-06"^^xsd:date .


###  https://w3id.org/mod#numberOfAxioms
mod:numberOfAxioms
                    rdf:type                owl:DatatypeProperty ;
                    rdfs:subPropertyOf      mod:metrics ;
                    rdfs:label              "number of axioms or triples"@en ;
                    rdfs:domain             mod:SemanticArtefactDistribution ,
                                            mod:SemanticArtefactCatalog ;
					dct:domainIncludes	aowm:Distribution ,
											aowm:Catalog ;
                    rdfs:range              xsd:nonNegativeInteger ;
                    dct:description     "MOD: The total number of axioms in an ontology. OMV: Number of axioms in the ontology."@en ;
                    rdfs:isDefinedBy        <http://omv.ontoware.org/2005/05/ontology> ;
                    dct:issued          "2009-12-24"^^xsd:date ;
                    owl:equivalentProperty  omv:numberOfAxioms ,
                                            <http://www.isibang.ac.in/ns/mod/1.0/noOfAxioms> .


###  https://w3id.org/mod#numberOfLabels
mod:numberOfLabels
                    rdf:type                owl:DatatypeProperty ;
                    rdfs:subPropertyOf      mod:metrics ;
                    rdfs:label              "number of data properties"@en ;
                    rdfs:domain             mod:SemanticArtefactDistribution ,
                                            mod:SemanticArtefactCatalog ;
					dct:domainIncludes	aowm:Distribution ,
											aowm:Catalog ;
                    rdfs:range              xsd:nonNegativeInteger ;
                    dct:description     "MOD: Number of defined labels for any resources in an ontology (classes, properties, etc)."@en ;
                    rdfs:isDefinedBy        <https://w3id.org/mod> ;
                    dct:issued          "2017-07-06"^^xsd:date .

###  https://w3id.org/mod#numberOfDeprecated
mod:numberOfDeprecated
                    rdf:type                owl:DatatypeProperty ;
                    rdfs:subPropertyOf      mod:metrics ;
                    rdfs:label              "number of deprecated objects"@en ;
                    rdfs:domain             mod:SemanticArtefactDistribution ,
                                            mod:SemanticArtefactCatalog ;
					dct:fomainIncludes	aowm:Distribution ,
											aowm:Catalog ;
                    rdfs:range              xsd:nonNegativeInteger ;
                    dct:description     "MOD: Number of objects (classes, properties, etc) declared as owl:deprecated=true in an ontology."@en ;
                    rdfs:isDefinedBy        <https://w3id.org/mod> ;
                    dct:issued          "2024-05-30"^^xsd:date .


### http://www.w3.org/ns/dcat#byteSize
dcat:byteSize       rdf:type                rdf:Property , owl:DatatypeProperty ;
                    rdfs:label              "byte size"@en ;
                    rdfs:domain             dcat:Distribution ;
					dct:domainIncludes	aowm:Distribution ;
                    rdfs:range              rdfs:Literal ;
                    dct:description     "DCAT: The size of a distribution in bytes. MOD: The byte size of an ontology."@en ;
                    rdfs:isDefinedBy        <http://www.w3.org/TR/vocab-dcat/> ;
                    dct:issued          "2014-01-16"^^xsd:date ;
                    owl:equivalentProperty  <http://www.isibang.ac.in/ns/mod/1.0/size> ,
                                            <http://www.isibang.ac.in/ns/mod/1.0/byteSize> .

###  https://w3id.org/mod#maxDepth
mod:maxDepth        rdf:type                owl:DatatypeProperty ;
                    rdfs:subPropertyOf      mod:metrics ;
                    rdfs:label              "maximum depth of the hierachy"@en ;
                    rdfs:domain             mod:SemanticArtefactDistribution ;
					dct:domainIncludes	aowm:Distribution ;
                    rdfs:range              xsd:nonNegativeInteger ;
                    dct:description     "MOD: Maximum depth of the hierarchy tree (BioPortal definition)."@en ;
                    rdfs:isDefinedBy        <https://w3id.org/mod> ;
                    dct:issued          "2017-07-06"^^xsd:date .


###  https://w3id.org/mod#maxChildCount
mod:maxChildCount   rdf:type                owl:DatatypeProperty ;
                    rdfs:subPropertyOf      mod:metrics ;
                    rdfs:label              "maximum number of children per class"@en ;
                    rdfs:domain             mod:SemanticArtefactDistribution ;
					dct:domainIncludes	aowm:Distribution ;
                    rdfs:range              xsd:nonNegativeInteger ;
                    dct:description     "MOD: Maximum number of children per class (BioPortal definition)."@en ;
                    rdfs:isDefinedBy        <https://w3id.org/mod> ;
                    dct:issued          "2017-07-06"^^xsd:date .


###  https://w3id.org/mod#averageChildCount
mod:averageChildCount
                    rdf:type                owl:DatatypeProperty ;
                    rdfs:subPropertyOf      mod:metrics ;
                    rdfs:label              "average number of children per class"@en ;
                    rdfs:domain             mod:SemanticArtefactDistribution ;
					dct:domainIncludes	aowm:Distribution ;
                    rdfs:range              xsd:decimal ;
                    dct:description     "MOD: Average number of children per class (BioPortal definition)."@en ;
                    rdfs:isDefinedBy        <https://w3id.org/mod> ;
                    dct:issued          "2017-07-06"^^xsd:date .


###  https://w3id.org/mod#classesWithOneChild
mod:classesWithOneChild
                    rdf:type                owl:DatatypeProperty ;
                    rdfs:subPropertyOf      mod:metrics ;
                    rdfs:label              "number of classes with a single child"@en ;
                    rdfs:domain             mod:SemanticArtefactDistribution ;
					dct:domainIncludes	aowm:Distribution ;
                    rdfs:range              xsd:nonNegativeInteger ;
                    dct:description     "MOD: Number of classes that have only one subclass in the is-a hierarchy (BioPortal definition)."@en ;
                    rdfs:isDefinedBy        <https://w3id.org/mod> ;
                    dct:issued          "2017-07-06"^^xsd:date . 


###  https://w3id.org/mod#classesWithMoreThan25Children
mod:classesWithMoreThan25Children
                    rdf:type                owl:DatatypeProperty ;
                    rdfs:subPropertyOf      mod:metrics ;
                    rdfs:label              "number of classes with more than 25 children"@en ;
                    rdfs:domain             mod:SemanticArtefactDistribution ;
					dct:domainIncludes	aowm:Distribution ;
                    rdfs:range              xsd:nonNegativeInteger ;
                    dct:description     "MOD: Number of classes that have more than 25 direct subclasses (BioPortal definition)."@en ;
                    rdfs:isDefinedBy        <https://w3id.org/mod> ;
                    dct:issued          "2017-07-06"^^xsd:date .


###  https://w3id.org/mod#classesWithNoDefinition
mod:classesWithNoDefinition
                    rdf:type                owl:DatatypeProperty ;
                    rdfs:subPropertyOf      mod:metrics ;
                    rdfs:label              "number of classes with no definition"@en ;
                    rdfs:domain             mod:SemanticArtefactDistribution ;
					dct:domainIncludes	aowm:Distribution ;
                    rdfs:range              xsd:nonNegativeInteger ;
                    dct:description     "MOD: Number of classes that have no value for the definition property (BioPortal definition). For ontologies in OBO and RRF formats, the property for definition is part of the language. For OWL ontologies, the authors specify this property as part of the ontology metadata (the default is skos:definition)."@en ;
                    rdfs:isDefinedBy        <https://w3id.org/mod> ;
                    dct:issued          "2017-07-06"^^xsd:date .

###  https://w3id.org/mod#classesWithNoFormalDefinition
mod:classesWithNoFormalDefinition
                    rdf:type                owl:DatatypeProperty ;
                    rdfs:subPropertyOf      mod:metrics ;
                    rdfs:label              "number of classes with no formal or logical definition"@en ;
                    rdfs:domain             mod:SemanticArtefactDistribution ;
					dct:domainIncludes	aowm:Distribution ;
                    rdfs:range              xsd:nonNegativeInteger ;
                    dct:description     "MOD: Number of classes with no formal or logical definition (e.g., an OWL restriction)."@en ;
                    rdfs:isDefinedBy        <https://w3id.org/mod> ;
                    dct:issued          "2024-05-30"^^xsd:date .


###  https://w3id.org/mod#classesWithNoLabel
mod:classesWithNoLabel
                    rdf:type                owl:DatatypeProperty ;
                    rdfs:subPropertyOf      mod:metrics ;
                    rdfs:label              "number of classes with no label"@en ;
                    rdfs:domain             mod:SemanticArtefactDistribution ;
					dct:domainIncludes	aowm:Distribution ;
                    rdfs:range              xsd:nonNegativeInteger ;
                    dct:description     "MOD: Number of classes with no labels."@en ;
                    rdfs:isDefinedBy        <https://w3id.org/mod> ;
                    dct:issued          "2024-05-30"^^xsd:date .


###  https://w3id.org/mod#classesWithNoAuthorMetadata
mod:classesWithNoAuthorMetadata
                    rdf:type                owl:DatatypeProperty ;
                    rdfs:subPropertyOf      mod:metrics ;
                    rdfs:label              "number of classes with no author metadata"@en ;
                    rdfs:domain             mod:SemanticArtefactDistribution ;
					dct:domainIncludes	aowm:Distribution ;
                    rdfs:range              xsd:nonNegativeInteger ;
                    dct:description     "MOD: Number of classes with no author metadata."@en ;
                    rdfs:isDefinedBy        <https://w3id.org/mod> ;
                    dct:issued          "2024-05-30"^^xsd:date .


###  https://w3id.org/mod#classesWithNoDateMetadata
mod:classesWithNoDateMetadata
                    rdf:type                owl:DatatypeProperty ;
                    rdfs:subPropertyOf      mod:metrics ;
                    rdfs:label              "number of classes with no date metadata"@en ;
                    rdfs:domain             mod:SemanticArtefactDistribution ;
					dct:domainIncludes	aowm:Distribution ;
                    rdfs:range              xsd:nonNegativeInteger ;
                    dct:description     "MOD: Number of classes with no date metadata."@en ;
                    rdfs:isDefinedBy        <https://w3id.org/mod> ;
                    dct:issued          "2024-05-30"^^xsd:date .


###  https://w3id.org/mod#numberOfNotes
mod:numberOfNotes   rdf:type                owl:DatatypeProperty ;
                    rdfs:subPropertyOf      mod:metrics ;
                    rdfs:label              "number of notes or comments"@en ;
                    rdfs:domain             mod:SemanticArtefact ;
					dct:domainIncludes	aowm:Ontology ;
                    rdfs:range              xsd:nonNegativeInteger ;
                    dct:description     "MOD: Number of notes or comments (maybe represented with schema:comment) related to the ontologies."@en ;
                    rdfs:isDefinedBy        <https://w3id.org/mod> ;
                    dct:issued          "2024-05-30"^^xsd:date .


###  https://w3id.org/mod#numberOfUsingProjects
mod:numberOfUsingProjects
                    rdf:type                owl:DatatypeProperty ;
                    rdfs:subPropertyOf      mod:metrics ;
                    rdfs:label              "number of using projects"@en ;
                    rdfs:domain             mod:SemanticArtefact ,
                                            mod:SemanticArtefactCatalog ;
					dct:domainIncludes	aowm:Ontology ,
											aowm:Catalog ;
                    rdfs:range              xsd:nonNegativeInteger ;
                    dct:description     "MOD: Number of projects (maybe represented with mod:usedInProject) using an ontology."@en ;
                    rdfs:isDefinedBy        <https://w3id.org/mod> ;
                    dct:issued          "2024-05-30"^^xsd:date .


###  https://w3id.org/mod#numberOfEndorsements
mod:numberOfEndorsements
                    rdf:type                owl:DatatypeProperty ;
                    rdfs:subPropertyOf      mod:metrics ;
                    rdfs:label              "number of endorsements"@en ;
                    rdfs:domain             mod:SemanticArtefact ,
                                            mod:SemanticArtefactCatalog ;
					dct:domainIncludes	aowm:Ontology ,
											aowm:Catalog ;
                    rdfs:range              xsd:nonNegativeInteger ;
                    dct:description     "MOD: Number of endorsing organizations (maybe represented with mod:endorsedBy)."@en ;
                    rdfs:isDefinedBy        <https://w3id.org/mod> ;
                    dct:issued          "2024-05-30"^^xsd:date .


###  https://w3id.org/mod#numberOfEvaluations
mod:numberOfEvaluations
                    rdf:type                owl:DatatypeProperty ;
                    rdfs:subPropertyOf      mod:metrics ;
                    rdfs:label              "number of evaluations"@en ;
                    rdfs:domain             mod:SemanticArtefact ;
					dct:domainIncludes	aowm:Ontology ;
                    rdfs:range              xsd:nonNegativeInteger ;
                    dct:description     "MOD: Number of evaluations (maybe represented with mod:hasEvaluation)."@en ;
                    rdfs:isDefinedBy        <https://w3id.org/mod> ;
                    dct:issued          "2024-05-30"^^xsd:date .


###  https://w3id.org/mod#fairScore
mod:fairScore       rdf:type                owl:DatatypeProperty ;
                    rdfs:subPropertyOf      mod:metrics ;
                    rdfs:label              "FAIR score"@en ;
                    rdfs:domain             mod:SemanticArtefactDistribution ,
                                            mod:SemanticArtefactCatalog ;
					dct:domainIncludes	aowm:Distribution ,
											aowm:Catalog;
                    rdfs:range              xsd:nonNegativeInteger ;
                    dct:description     "MOD: Latest FAIR score the semantic artefact or average FAIR score of all resources in the catalogue, obtained with a known or identified FAIRness assessment tool."@en ;
                    rdfs:isDefinedBy        <https://w3id.org/mod> ;
                    dct:issued          "2024-05-30"^^xsd:date .


###  https://w3id.org/mod#numberOfMappings
mod:numberOfMappings
                    rdf:type                owl:DatatypeProperty ;
                    rdfs:subPropertyOf      mod:metrics ;
                    rdfs:label              "number of mappings"@en ;
                    rdfs:domain             mod:SemanticArtefactDistribution ,
                                            mod:SemanticArtefactCatalog;
					dct:domainIncludes	aowm:Distribution ,
											aowm:Catalog ;
                    rdfs:range              xsd:nonNegativeInteger ;
                    dct:description     "MOD: Number of mappings within a given semantic artefact or semantic artefact catalogue."@en ;
                    rdfs:isDefinedBy        <https://w3id.org/mod> ;
                    dct:issued          "2024-06-25"^^xsd:date .


###  https://w3id.org/mod#numberOfUsers
mod:numberOfUsers   rdf:type                owl:DatatypeProperty ;
                    rdfs:subPropertyOf      mod:metrics ;
                    rdfs:label              "number of users"@en ;
                    rdfs:domain             mod:SemanticArtefact ,
                                            mod:SemanticArtefactCatalog;
					dct:domainIncludes	aowm:Ontology ,
											aowm:Catalog ;
                    rdfs:range              xsd:nonNegativeInteger ;
                    dct:description     "MOD: Total number of users in a semantic artefact catalogue or number of users watching/following/using a given semantic artefact."@en ;
                    rdfs:isDefinedBy        <https://w3id.org/mod> ;
                    dct:issued          "2024-06-25"^^xsd:date .


###  https://w3id.org/mod#numberOfAgents
mod:numberOfAgents  rdf:type                owl:DatatypeProperty ;
                    rdfs:subPropertyOf      mod:metrics ;
                    rdfs:label              "number of agents"@en ;
                    rdfs:domain             mod:SemanticArtefact ,
                                            mod:SemanticArtefactCatalog;
					dct:domainIncludes	aowm:Ontology ,
											aowm:Catalog ;
                    rdfs:range              xsd:nonNegativeInteger ;
                    dct:description     "MOD: Total number of agents in a semantic artefact catalogue or number of agents related a given semantic artefact."@en ;
                    rdfs:isDefinedBy        <https://w3id.org/mod> ;
                    dct:issued          "2024-06-25"^^xsd:date .


###  https://w3id.org/mod#numberOfArtefacts
mod:numberOfArtefacts
                    rdf:type                owl:DatatypeProperty ;
                    rdfs:subPropertyOf      mod:metrics ;
                    rdfs:label              "number of semantic artefacts"@en ;
                    rdfs:domain             mod:SemanticArtefactCatalog ;
					dct:domainIncludes	aowm:Catalog ;
                    rdfs:range              xsd:nonNegativeInteger ;
                    dct:description     "MOD: Total number of semantic artefacts within a catalog."@en ;
                    rdfs:isDefinedBy        <https://w3id.org/mod> ;
                    dct:issued          "2024-06-25"^^xsd:date .




####media properties####
### http://schema.org/associatedMedia
schema:associatedMedia
                    rdf:type                rdf:Property ;
                    rdfs:label              "associated media"@en ;
                    dct:domainIncludes  aowm:Ontology ,
                                            aowm:Catalog ;
                    dct:description     "SCHEMA: A media object that encodes this CreativeWork. This property is a synonym for encoding."@en ;
                    rdfs:isDefinedBy        <http://schema.org/> ;
                    dct:issued          "2012-04-21"^^xsd:date .


### http://xmlns.com/foaf/0.1/depiction
foaf:depiction      rdf:type                rdf:Property , owl:ObjectProperty ;
                    rdfs:label              "depiction"@en ;
                    rdfs:domain             owl:Thing ;
                    dct:domainIncludes  aowm:Ontology ,
                                            aowm:Catalog ;
                    rdfs:range              foaf:Image ;
                    dct:description     "FOAF: A depiction of some thing. DOAP: Web page with screenshots of project. An image of the item. This can be a URL or a fully described ImageObject."@en ;
                    rdfs:isDefinedBy        <http://xmlns.com/foaf/0.1/> ;
                    dct:issued          "2014-01-14"^^xsd:date ;
                    owl:equivalentProperty  schema:image ,
                                            doap:screenshots .
                    

### http://xmlns.com/foaf/0.1/logo
foaf:logo           rdf:type                rdf:Property , owl:InverseFunctionalProperty , owl:ObjectProperty  ;
                    rdfs:label              "logo"@en ;
                    rdfs:domain             owl:Thing ;
                    dct:domainIncludes  aowm:Ontology ,
                                            aowm:Catalog ;
                    rdfs:range              owl:Thing ;
                    dct:description     "FOAF: A logo representing some thing. SCHEMA: An associated logo."@en ;
                    rdfs:isDefinedBy        <http://xmlns.com/foaf/0.1/> ;
                    dct:issued          "2014-01-14"^^xsd:date ;
                    owl:equivalentProperty  schema:logo .
					
aowm:visualization
	a owl:ObjectProperty ;
	rdfs:subPropertyOf schema:image ;
	rdfs:domain aowm:Ontology ;
	rdfs:range schema:ImageObject ;
	rdfs:label "Visualization"@en ;
	dct:description "Visualization of an ontology."@en ;
    rdfs:isDefinedBy <http://dqm.faw.jku.at/ontologies/aowm> .
                   
####usage and application context properties####
###  https://w3id.org/mod#knownUsage
mod:knownUsage      rdf:type                owl:DatatypeProperty ;
                    rdfs:label              "known usage"@en ;
                    rdfs:domain             mod:SemanticArtefact ,
                                            mod:SemanticArtefactCatalog ;
					dct:domainIncludes		aowm:Ontology ,
											aowm:Catalog ;
                    rdfs:range              mod:string ;
                    dct:description     "OMV: The applications where the ontology is being used."@en ;
                    rdfs:isDefinedBy        <http://omv.ontoware.org/2005/05/ontology> ;
                    dct:issued          "2009-12-24"^^xsd:date ;
                    owl:equivalentProperty  omv:knownUsage .
    

### https://w3id.org/mod#designedForTask
mod:designedForTask rdf:type                owl:ObjectProperty ;
                    rdfs:label              "designed for task"@en ;
                    rdfs:domain             mod:SemanticArtefact ;
					dct:domainIncludes		aowm:Ontoloy ;
                    rdfs:range              mod:SemanticArtefactTask ;
                    dct:description     "OMV: The purpose for which the ontology was originally designed."@en ;
                    rdfs:isDefinedBy        <http://omv.ontoware.org/2005/05/ontology> ;
                    dct:issued          "2009-12-24"^^xsd:date .


### http://purl.org/dc/terms/subject
dct:subject     rdf:type                rdf:Property ;
                    rdfs:subPropertyOf      dc:subject ;
                    rdfs:label              "subject"@en ;
                    dct:domainIncludes  	aowm:Ontology ,
                                            aowm:Catalog ;
                    dct:description     "dct: The topic of the resource. OMV: Typically, the domain can refer to established topic hierarchies such as the general purpose topic hierarchy DMOZ or the domain specific topic hierarchy ACM for the computer science domain. SCHEMA: The subject matter of the content. DCAT: A main category of the resource. A resource can have multiple themes. FOAF: A topic of some page or document."@en ;
                    rdfs:isDefinedBy        <http://purl.org/dc/terms/> ;
                    dct:issued          "2008-01-14"^^xsd:date ;
                    owl:equivalentProperty  omv:hasDomain ,
                                            schema:about ,
                                            dcat:theme ,
                                            foaf:topic .


### http://purl.org/dc/terms/coverage
dct:coverage    rdf:type                rdf:Property ;
                    rdfs:subPropertyOf      dc:coverage ;
                    rdfs:label              "coverage"@en ;
                    dct:domainIncludes  aowm:Ontology ,
                                            aowm:Catalog ;
                    dct:description     "dct: The spatial or temporal topic of the resource, the spatial applicability of the resource, or the jurisdiction under which the resource is relevant. Spatial topic and spatial applicability may be a named place or a location specified by its geographic coordinates. Temporal topic may be a named period, date, or date range. A jurisdiction may be a named administrative entity or a geographic place to which the resource applies. Recommended practice is to use a controlled vocabulary such as the Getty Thesaurus of Geographic Names [[TGN](https://www.getty.edu/research/tools/vocabulary/tgn/index.html)]. Where appropriate, named places or time periods may be used in preference to numeric identifiers such as sets of coordinates or date ranges.  Because coverage is so broadly defined, it is preferable to use the more specific subproperties Temporal Coverage and Spatial Coverage."@en ;
                    rdfs:isDefinedBy        <http://purl.org/dc/terms/> ;
                    dct:issued          "2008-01-14"^^xsd:date .


### http://www.w3.org/ns/adms#supportedSchema
adms:supportedSchema
                    rdf:type                rdf:Property , owl:ObjectProperty ;
                    rdfs:label              "supported schema/format"@en ;
                    dct:domainIncludes  aowm:Catalog ;
                    rdfs:range              adms:Asset ;
                    dct:description     "ADMS: A schema according to which the Asset Repository can provide data about its content. SCHEMA: Media type, typically MIME format (see IANA site) of the content."@en ;
                    rdfs:isDefinedBy        <http://www.w3.org/TR/vocab-adms> ;
                    dct:issued          "2013-08-01"^^xsd:date .

### https://vocab.org/vann/example
vann:example        rdf:type                owl:AnnotationProperty ;
                    rdfs:subPropertyOf      rdfs:seeAlso ;
                    rdfs:label              "example"@en ;
                    dct:domainIncludes  aowm:Ontology ,
                                            aowm:Catalog ;
                    dct:description     "VANN: A reference to a resource that provides an example of how this resource can be used. SCHEMA: Example/instance/realization/derivation of the concept of this creative work. eg. The paperback edition, first edition, or eBook."@en ;
                    rdfs:isDefinedBy        <http://purl.org/vocab/vann/> ;
                    dct:issued          "2005-04-01"^^xsd:date ;
                    owl:equivalentProperty  schema:workExample .
				

aowm:frequencyOfUse
	a owl:DatatypeProperty ;
	rdfs:label "Frequency Of Use"@en ;
	rdfs:domain aowm:Ontology ;
	rdfs:range xsd:string ;
	dct:description: "Frequency of use of an ontology"@en ;
	dct:issued          "2026-01-30"^^xsd:date ;
	rdfs:isDefinedBy <http://dqm.faw.jku.at/ontologies/aowm> .
	
aowm:intendedUse
	a owl:DatatypeProperty ;
	rdfs:label "Intended Use"@en ;
	rdfs:domain aowm:Ontology ;
	rdfs:range xsd:string ;
	dct:description: "Intended use of an ontology."@en ;
	dct:issued          "2026-02-01"^^xsd:date ;
	rdfs:isDefinedBy <http://dqm.faw.jku.at/ontologies/aowm> .
	
aowm:validInContext
	a owl:DatatypeProperty ;
	rdfs:label "Valid Context"@en ;
	rdfs:domain aowm:Ontology ;
	rdfs:range xsd:string ;
	dct:description: "Valid only under certain conditions."@en ;
	dct:issued          "2026-02-01"^^xsd:date ;
	rdfs:isDefinedBy <http://dqm.faw.jku.at/ontologies/aowm> .
	
aowm:scopeOfValidity
	a owl:DatatypeProperty ;
	rdfs:label "Validity Scope"@en ;
	rdfs:domain aowm:Ontology ;
	rdfs:range xsd:string ;
	dct:description: "Scope of application in terms of subject matter or time."@en ;
	dct:issued          "2026-02-01"^^xsd:date ;
	rdfs:isDefinedBy <http://dqm.faw.jku.at/ontologies/aowm> .
	
aowm:assumption
	a owl:DatatypeProperty ;
	rdfs:label "Assumption"@en ;
	rdfs:domain aowm:Ontology ;
	rdfs:range xsd:string ;
	dct:description: "Explicit assumptions under which the resource is valid."@en ;
	dct:issued          "2026-02-01"^^xsd:date ;
	rdfs:isDefinedBy <http://dqm.faw.jku.at/ontologies/aowm> .
	
####person and organization properties####
### https://www.w3.org/ns/dcat#contactPoint
dcat:contactPoint   rdf:type                rdf:Property ,
                                            owl:ObjectProperty ;
                    rdfs:label              "contact point"@en ;
                    dct:domainIncludes 		aowm:Ontology ,
                                            aowm:Catalog ;
                    rdfs:range              vcard:Kind ;
                    dct:description     "DCAT: Relevant contact information for the cataloged resource. Use of vCard is recommended. SCHEMA: A maintainer of a Dataset, software package (SoftwareApplication), or other Project. A maintainer is a Person or Organization that manages contributions to, and/or publication of, some (typically complex) artifact. It is common for distributions of software and data to be based on 'upstream' sources." ;
                    rdfs:isDefinedBy        <http://www.w3.org/TR/vocab-dcat/> ;
                    dct:issued          "2014-01-16"^^xsd:date ;
                    owl:equivalentProperty  schema:maintainer .

    
### http://purl.org/dc/terms/creator
dct:creator     rdf:type                rdf:Property ;
                    rdfs:subPropertyOf      dc:creator , dct:contributor ;
                    rdfs:label              "creator"@en ;
                    dct:domainIncludes  aowm:Ontology ,
                                        aowm:Catalog ;
					dct:rangeIncludes	aowm:Agent ;
                    dct:description     "OMV: Main responsible for the creation of the ontology. dct: An entity primarily responsible for making the resource. FOAF: An agent that made this thing. PROV: Attribution is the ascribing of an entity to an agent. PAV:authoredBy: An agent that originated or gave existence to the work that is expressed by the digital resource.PAV:createdBy: An agent primary responsible for making the digital artifact or resource representation. DOAP: Maintainer of a project, a project leader. SCHEMA:author: The author of this content or rating. SCHEMA:creator: The creator/author of this CreativeWork. DCAT: The entity responsible for producing the resource."@en ;
                    rdfs:isDefinedBy        <http://purl.org/dc/terms/> ;
                    dct:issued          "2008-01-14"^^xsd:date ;
                    owl:equivalentProperty  omv:creator ,
                                            pav:authoredBy ,
                                            pav:createdBy ,
                                            schema:author ,
                                            doap:maintainer ,
                                            prov:wasAttributedTo ,
                                            foaf:maker .


### http://purl.org/dc/terms/contributor
dct:contributor rdf:type                rdf:Property ;
                    rdfs:subPropertyOf      dc:contributor ;
                    rdfs:label              "contributor"@en ;
                    dct:domainIncludes  aowm:Ontology ,
                                            aowm:Catalog ;
					dct:rangeIncludes	aowm:Agent ;
                    dct:description     "dct: An entity responsible for making contributions to the resource. OMV: Contributors to the creation of the ontology. PAV: The resource was contributed to by the given agent. SCHEMA: A secondary contributor to the CreativeWork or Event. DOAP: Project contributor."@en ;
                    rdfs:isDefinedBy        <http://purl.org/dc/terms/> ;
                    dct:issued          "2008-01-14"^^xsd:date ;
                    owl:equivalentProperty  omv:hasContributor ,
                                            pav:contributedBy ,
                                            schema:contributor ,
                                            doap:developer ,
                                            doap:helper ,
                                            oboinowl:saved-by ,
                                            oboinowl:savedBy .


### http://purl.org/pav/curatedBy
pav:curatedBy       rdf:type                owl:ObjectProperty ;
                    rdfs:subPropertyOf      pav:contributedBy ;
                    rdfs:label              "curator"@en ,
                                            "curateur"@fr ;
                    dct:domainIncludes  aowm:Ontology ,
                                            aowm:Catalog ,
                                            aowm:CatalogRecord ;
					dct:rangeIncludes	aowm:Agent ;
                    dct:description     "PAV: Specifies an agent specialist responsible for shaping the expression in an appropriate format. Often the primary agent responsible for ensuring the quality of the representation. MOD: A curator who restructures the previously authored content and shapes it to be appropriate for the intended representation (e.g. by normalizing the fields for being represented in a spreadsheet). "@en ;
                    rdfs:isDefinedBy        <http://purl.org/pav/> ;
                    dct:issued          "2014-08-28"^^xsd:date .


### http://schema.org/translator
schema:translator   rdf:type                rdf:Property ;
                    rdfs:label              "translator"@en ;
                    dct:domainIncludes  aowm:Ontology ,
                                            aowm:Catalog ;
					dct:rangeIncludes	aowm:Agent ;
                    dct:description     "SCHEMA: Organization or person who adapts a creative work to different languages, regional differences and technical requirements of a target market, or that translates during some event."@en ;
                    rdfs:isDefinedBy        <http://schema.org/> ;
                    dct:issued          "2012-04-21"^^xsd:date .        


### http://purl.org/dc/terms/publisher
dct:publisher   rdf:type                rdf:Property ;
                    rdfs:subPropertyOf      dc:publisher ;
                    rdfs:label              "publisher"@en ;
                    dct:domainIncludes  aowm:Ontology ,
                                            aowm:Catalog ;
					dct:rangeIncludes	aowm:Agent ;
                    dct:description     "dct: An entity responsible for making the resource available. SCHEMA: The publisher of creative work. SCHEMA: The Organization on whose behalf the creator was working. SCHEMA: The service provider, service operator, or service performer; the goods producer. Another party (a seller) may offer those services or goods on behalf of the provider. A provider may also serve as the seller. ADMS: The name of the agency that issued the identifier. DCAT: The entity responsible for making the item available."@en ;                    rdfs:isDefinedBy        <http://purl.org/dc/terms/> ;
                    dct:issued          "2008-01-14"^^xsd:date ;
                    owl:equivalentProperty  schema:publisher ,
                                            schema:sourceOrganization ,
                                            schema:provider ,
                                            adms:schemaAgency .


### http://xmlns.com/foaf/0.1/fundedBy
foaf:fundedBy       rdf:type                rdf:Property , owl:ObjectProperty ;
                    rdfs:label              "funded or sponsored by"@en ;
                    rdfs:domain             owl:Thing ;
                    dct:domainIncludes  aowm:Ontology ,
                                            aowm:Catalog ;
                    rdfs:range              owl:Thing ;
                    dct:description     "MOD: An ontology that is sponsored by and developed under a project. FOAF: An organization funding a project or person. SCHEMA: A person or organization that supports (sponsors) something through some kind of financial contribution."@en ;
                    rdfs:isDefinedBy        <http://xmlns.com/foaf/0.1/> ;
                    dct:issued          "2014-01-14"^^xsd:date ;
                    owl:equivalentProperty  schema:funder , 
                                            <http://www.isibang.ac.in/ns/mod/1.0/sponsoredBy> .


### http://schema.org/funding
schema:funding      rdf:type                rdf:Property ;
                    rdfs:label              "funding"@en ;
                    dct:domainIncludes  aowm:Ontology ,
                                            aowm:Catalog ;
                    dct:description     "SCHEMA: A Grant that directly or indirectly provide funding or sponsorship for this item."@en ;
                    rdfs:isDefinedBy        <http://schema.org/> ;
                    dct:issued          "2022-03-17"^^xsd:date ;
                    owl:equivalentProperty  schema:funder , 
                                            <http://www.isibang.ac.in/ns/mod/1.0/sponsoredBy> .


###  https://w3id.org/mod#endorsedBy
mod:endorsedBy      rdf:type                owl:ObjectProperty ;
                    rdfs:label              "endorsed by"@en ;
                    rdfs:domain             aowm:Ontology ,
                                            aowm:Catalog ;
                    rdfs:range              rdfs:Literal ;
                    dct:description     "MOD: An ontology endorsed by an agent. OMV: The parties that have expressed support or approval to this ontology."@en ;
                    rdfs:isDefinedBy        <http://omv.ontoware.org/2005/05/ontology> ;
                    dct:issued          "2009-12-24"^^xsd:date ;
                    owl:equivalentProperty  omv:endorsedBy .


### http://www.w3.org/ns/prov#qualifiedAttribution
prov:qualifiedAttribution 
                    rdf:type                owl:ObjectProperty ;
                    rdfs:subPropertyOf      prov:qualifiedInfluence ;
                    rdfs:label              "qualified attribution"@en ;
                    rdfs:domain             prov:Entity ;
                    dct:domainIncludes  aowm:Ontolgoy ,
                                            aowm:Catalog ;
                    rdfs:range              prov:Attribution ;
                    dct:description     "PROV: Attribution is the ascribing of an entity to an agent. When an entity e is attributed to agent ag, entity e was generated by some unspecified activity that in turn was associated to agent ag. Thus, this relation is useful when the activity is not known, or irrelevant. DCAT: Link to an Agent having some form of responsibility for the resource."@en ;
                    rdfs:isDefinedBy        <http://www.w3.org/ns/prov-o#> ;
                    dct:issued          "2013-04-30"^^xsd:date .

####community properties####
### http://schema.org/comment
schema:comment      rdf:type                rdf:Property ;
                    rdfs:label              "user notes or reviews"@en ,
                                            "commentaires ou avis d'utilisateurs"@fr ;
                    dct:domainIncludes  aowm:Ontology ,
                                            aowm:Catalog ;
                    dct:description     "SCHEMA: Comments, typically from users."@en ;
                    rdfs:isDefinedBy        <http://schema.org/> ;
                    dct:issued          "2012-04-21"^^xsd:date ;
                    pav:derivedFrom         <https://w3id.org/mod/1.4> ;
                    pav:importedOn          "2018-08-02"^^xsd:date ;
                    
            #OPTIONAL STATEMENTS
                    prov:wasInfluencedBy    "FAIR principle: F4, A1.1, A1.2" ;
            
            #OTHER ORIGINAL STATEMENTS IF ANY 
                    schema:domainIncludes   schema:CreativeWork ;
                    schema:rangeIncludes    schema:Comment .
    

### https://w3id.org/mod#hasEvaluation
mod:hasEvaluation   rdf:type                owl:ObjectProperty ;
                    rdfs:label              "evaluation"@en ;
					rdfs:domain             mod:SemanticArtefact ;
                    dct:domainIncludes      aowm:Ontology ;
                    rdfs:range              mod:Evaluation ;
                    dct:description     "MOD: This property makes a relationship between an ontology and its evaluation result."@en ; 
                    rdfs:isDefinedBy        <https://w3id.org/mod> ;
                    dct:issued          "2015-08-05"^^xsd:date ;
                    owl:equivalentProperty  schema:review .


### https://w3id.org/mod#group
mod:group           rdf:type                owl:ObjectProperty ;
                    rdfs:label              "group"@en ;
					rdfs:domain             mod:SemanticArtefact ,
                                            mod:SemanticArtefactCatalog ;
                    dct:domainIncludes      aowm:Ontology ,
                                            aowm:Catalog ;
                    rdfs:range              mod:Group ;
                    dct:description     "MOD: A group of semantic artefacts that the given semantic artefact is usually considered within or a group hosted/served/represented by the given semantic artefact catalogue."@en ;
                    rdfs:isDefinedBy        <https://w3id.org/mod> ;
                    dct:issued          "2017-07-06"^^xsd:date .
            

### https://w3id.org/mod#usedInProject
mod:usedInProject   rdf:type                owl:ObjectProperty ;
                    rdfs:label              "used in project"@en ;
					rdfs:domain             mod:SemanticArtefact ,
                                            mod:SemanticArtefactCatalog ;
                    dct:domainIncludes       aowm:Ontology ,
                                            aowm:Catalog ;
                    rdfs:range              foaf:Project ;
                    dct:description     "MOD: An ontology that is used in a project."@en ; 
                    rdfs:isDefinedBy        <https://w3id.org/mod> ;
                    dct:issued          "2015-08-05"^^xsd:date .


### http://purl.org/dc/terms/audience
dct:audience    rdf:type                rdf:Property ;
                    rdfs:subPropertyOf      dc:audience ;
                    rdfs:label              "target audience"@en ;
                    dct:domainIncludes  aowm:Ontology ,
                                            aowm:Catalog ;
                    dct:description     "dct: a class of entity for whom the resource is intended or useful (public vis ou recommand pour la ressource). DOAP: Description of target user base. SCHEMA: An intended audience, i.e. a group for whom something was created."@en ;
                    rdfs:isDefinedBy        <http://purl.org/dc/terms/> ;
                    dct:issued          "2001-05-21"^^xsd:date ; 
                    owl:equivalentProperty  doap:audience ,
                                            schema:audience .


### http://schema.org/publishingPrinciples
schema:publishingPrinciples
                    rdf:type                rdf:Property ;
                    rdfs:label              "publishing principles"@en ;
                    dct:domainIncludes  aowm:Catalog ;
                    dct:description     "SCHEMA: The publishingPrinciples property indicates (typically via URL) a document describing the editorial principles of an Organization (or individual, e.g. a Person writing a blog) that relate to their activities as a publisher, e.g. ethics or diversity policies."@en ;
                    rdfs:isDefinedBy        <http://schema.org/> ;
                    dct:issued          "2012-04-21"^^xsd:date .


### https://w3id.org/mod#analytics
mod:analytics       rdf:type                owl:ObjectProperty ;
                    rdfs:label              "analytics"@en ;
					rdfs:domain             mod:SemanticArtefact ,
                                            mod:SemanticArtefactCatalog ;
                    dct:domainIncludes  aowm:Ontology ,
                                            aowm:Catalog ;
                    rdfs:range              mod:Analytics ;
                    dct:description     "MOD: This property shall be used to store any analytics for an ontology. E.g., number of visits an ontology received in a portal, number of downloads, etc."@en ; 
                    rdfs:isDefinedBy        <https://w3id.org/mod> ;
                    dct:issued          "2018-08-02"^^xsd:date .
     

### http://usefulinc.com/ns/doap/repository
doap:repository     rdf:type                rdf:Property ;
                    rdfs:label              "repository"@en ;
                    rdfs:domain             doap:Project ;
                    dct:domainIncludes  aowm:Ontology ,
                                            aowm:Catalog ;
                    rdfs:range              doap:Repository ;
                    dct:description     "DOAP: Source code repository."@en ;
                    rdfs:isDefinedBy        <http://usefulinc.com/ns/doap#> ;
                    dct:issued          "2004"^^xsd:date .
            

### http://usefulinc.com/ns/doap/bug-database
doap:bug-database    rdf:type                rdf:Property ;
                    rdfs:label              "bug database"@en ;
                    rdfs:domain             doap:Project ;
                    dct:domainIncludes  aowm:Ontology ,
                                            aowm:Catalog ;
                    dct:description     "DOAP: Bug tracker for a project."@en ;
                    rdfs:isDefinedBy        <http://usefulinc.com/ns/doap#> ;
                    dct:issued          "2004"^^xsd:date .

            
### http://usefulinc.com/ns/doap/mailing-list
doap:mailing-list   rdf:type                rdf:Property ;
                    rdfs:label              "mailing list"@en ;
                    rdfs:domain             doap:Project ;
                    dct:domainIncludes  aowm:Ontology ,
                                            aowm:Catalog ;
                    dct:description     "DOAP: Mailing list home page or email address."@en ;
                    rdfs:isDefinedBy        <http://usefulinc.com/ns/doap#> ;
                    dct:issued          "2004"^^xsd:date .
            

### https://w3id.org/mod#toDoList
mod:toDoList        rdf:type                owl:ObjectProperty ;
                    rdfs:label              "to-do list"@en ;
                    dct:domainIncludes  aowm:Ontology ,
                                            aowm:Catalog ;
                    rdfs:range              <http://www.w3.org/2002/12/cal/ical#Vtodo> ;
                    dct:description     "VOID: Describes future tasks planned by a resource curator. This property is primarily intended to be used for vocabularies or datasets, but the domain is left open, it can be used for any resource. Use iCalendar Vtodo class and its properties to further describe the task calendar, priorities etc."@en ;    
                    rdfs:isDefinedBy        <http://purl.org/vocommons/voaf> ;
                    dct:issued          "2013-05-23"^^xsd:date ;
                    owl:equivalentProperty  voaf:toDoList .
            

### http://schema.org/award
schema:award        rdf:type                rdf:Property ;
                    rdfs:label              "award"@en ;
                    dct:domainIncludes  aowm:Ontology ,
                                            aowm:Catalog ;
                    dct:description     "SCHEMA: An award won by or for this item."@en ;
                    rdfs:isDefinedBy        <http://schema.org/> ;
                    dct:issued          "2012-04-21"^^xsd:date .


####links####
### http://www.w3.org/ns/dcat#accessURL
dcat:accessURL      rdf:type                rdf:Property , owl:ObjectProperty ;
                    rdfs:label              "access URL"@en ;
                    rdfs:domain             dcat:Distribution ;
					dct:domainIncludes  aowm:Distribution ,
                                            aowm:Catalog ;
                    rdfs:range              rdfs:Resource ;
                    dct:description     "DCAT: A URL of a resource that gives access to a distribution of the dataset. E.g. landing page, feed, SPARQL endpoint. Use for all cases except a simple download link, in which case downloadURL is preferred. OMV: The location where the ontology can be found. It should be accessible via a URL. It can be the same as the value for URI property. DOAP:  Web page from which the project software can be downloaded."@en ;
                    rdfs:isDefinedBy        <http://www.w3.org/TR/vocab-dcat/> ;
                    dct:issued          "2014-01-16"^^xsd:date ;
                    owl:equivalentProperty  omv:resourceLocator ,
                                            doap:download-page .
											
											
### http://purl.org/dc/terms/isFormatOf
dct:isFormatOf  rdf:type                rdf:Property ;
                    rdfs:subPropertyOf      dc:relation , dct:relation ;
                    rdfs:label              "is format of"@en ;
                    dct:domainIncludes  aowm:Ontology ;
                    dct:description     "dct: A related resource that is substantially the same as the described resource, but in another format."@en ;
                    rdfs:isDefinedBy        <http://purl.org/dc/terms/> ;
                    dct:issued          "2000-07-11"^^xsd:date ;
                    owl:equivalentProperty  schema:hasPart ,
                                            <http://www.isibang.ac.in/ns/mod/1.2/syntax> .
											
### http://purl.org/dc/terms/hasFormat
dct:hasFormat   rdf:type                rdf:Property ;
                    rdfs:subPropertyOf      dc:relation , dct:relation ;
                    rdfs:label              "has format"@en ;
                    dct:domainIncludes  aowm:Ontology ;
                    dct:description     "dct: A related resource that is substantially the same as the pre-existing described resource, but in another format."@en ;
                    rdfs:isDefinedBy        <http://purl.org/dc/terms/> ;
                    dct:issued          "2000-07-11"^^xsd:date ;
                    owl:equivalentProperty  schema:hasPart ,
                                            <http://www.isibang.ac.in/ns/mod/1.2/syntax> .
											
											
### http://www.w3.org/ns/dcat#downloadURL
dcat:downloadURL    rdf:type                rdf:Property , owl:ObjectProperty ;
                    rdfs:label              "download URL"@en ;
                    rdfs:domain             dcat:Distribution ;
                    dct:domainIncludes  aowm:Distribution ;
                    rdfs:range              rdfs:Resource ;
                    dct:description     "DCAT: The URL of the downloadable file in a given format. E.g. CSV file or RDF file. The format is indicated by the distribution's dct:format and/or dcat:mediaType. VOID: An RDF dump, partial or complete, of a void:Dataset. DOAP: Mirror of software download web page. SCHEMA: A downloadable form of this dataset, at a specific location, in a specific format."@en ; 
                    rdfs:isDefinedBy        <http://www.w3.org/TR/vocab-dcat/> ;
                    dct:issued          "2014-01-16"^^xsd:date ;
                    owl:equivalentProperty  void:dataDump ,
                                            doap:download-mirror ,
                                            schema:distribution .
											
### http://rdfs.org/ns/void#uriLookupEndpoint
void:uriLookupEndpoint
                    rdf:type                rdf:Property ;
                    rdfs:label              "URI lookup endpoint"@en ;
                    rdfs:domain             void:Dataset ;
                    dct:domainIncludes  aowm:Ontology ,
                                            aowm:Catalog ;
                    rdfs:range              xsd:anyURI ;
                    dct:description     "VOID: A protocol endpoint for simple URI lookups for a void:Dataset."@en ;
                    rdfs:isDefinedBy        <http://vocab.deri.ie/void> ;
                    dct:issued          "2010-01-26"^^xsd:date .
					
					
### http://rdfs.org/ns/void#openSearchDescription
void:openSearchDescription
                    rdf:type                rdf:Property ;
                    rdfs:label              "free-text search endpoint"@en ;
                    rdfs:domain             void:Dataset ;
                    dct:domainIncludes  aowm:Ontology ,
                                            aowm:Catalog ;
                    rdfs:range              foaf:Document ;
                    dct:description     "VOID: An OpenSearch description document for a free-text search service over a void:Dataset. DOAP: The URI of a web service endpoint where software as a service may be accessed."@en ;
                    rdfs:isDefinedBy        <http://vocab.deri.ie/void> ;
                    dct:issued          "2010-01-26"^^xsd:date .
					
###  https://w3id.org/mod#browsingUI
mod:browsingUI      rdf:type                owl:DatatypeProperty ;
                    rdfs:label              "browsing user interface"@en ;
                    rdfs:domain             aowm:Distribution ;
                    rdfs:range              xsd:anyURI ;
                    dct:description     "MOD: The user interface (URL) where the ontology may be browsed or searched."@en ;
                    rdfs:isDefinedBy        <https://w3id.org/mod> ;
                    dct:issued          "2017-07-06"^^xsd:date .

## http://purl.org/dc/terms/source
dct:source      rdf:type                rdf:Property ;
                    rdfs:subPropertyOf      dc:source , dct:relation ;
                    rdfs:label              "source"@en ;
                    dct:domainIncludes  aowm:Ontology ,
                                            aowm:Catalog ;
                    dct:description     "dct: A related resource from which the described resource is derived. MOD: The ontology(ies) referred to while creating the present ontology. PROV: Influence is the capacity of an entity, activity, or agent to have an effect on the character, development, or behavior of another by means of usage, start, end, generation, invalidation, communication, derivation, attribution, association, or delegation. PROV: A derivation is a transformation of an entity into another, an update of an entity resulting in a new one, or the construction of a new entity based on a pre-existing entity. PAV: Derived from a different resource. NKOS: A resource used as the source for a derivative resource."@en ;
                    rdfs:isDefinedBy        <http://purl.org/dc/terms/> ;
                    dct:issued          "2008-01-14"^^xsd:date ;
                    owl:equivalentProperty  schema:isBasedOn ,
                                            nkos:basedOn ,
                                            prov:wasDerivedFrom , 
                                            prov:wasInfluencedBy ,
                                            pav:derivedFrom ,
                                            <http://www.isibang.ac.in/ns/mod/1.0/sourceOntology> .


### http://www.w3.org/ns/sparql-service-description#endpoint
sd:endpoint         rdf:type                rdf:Property , owl:InverseFunctionalProperty ; 
                    rdfs:label              "SPARQL endpoint"@en ;
                    rdfs:domain             sd:Service ;
                    dct:domainIncludes  aowm:Distribution ,
                                            aowm:Catalog ;
                    dct:description     "SD: Relates an instance of sd:Service to a SPARQL endpoint that implements the SPARQL Protocol service for the service. The object of the sd:endpoint property is an IRI. VOID: A SPARQL protocol endpoint that allows SPARQL query access to a void:Dataset."@en ;
                    rdfs:isDefinedBy        <ttp://www.w3.org/ns/sparql-service-description> ;
                    dct:issued          "2013-03-21"^^xsd:date ;
                    owl:equivalentProperty  void:sparqlEndpoint .
            
                     
### http://schema.org/includedInDataCatalog
schema:includedInDataCatalog
                    rdf:type                rdf:Property ;
                    rdfs:label              "indexed or included in catalog or repository"@en ;
                    dct:domainIncludes  aowm:Ontology ;
                    dct:description     "SCHEMA: A data catalog which contains this dataset."@en ;
                    rdfs:isDefinedBy        <http://schema.org/> ;
                    dct:issued          "2016-05-04"^^xsd:date .
					
					
					
####date properties####
### http://purl.org/dc/terms/created
dct:created     rdf:type                rdf:Property ;
                    rdfs:subPropertyOf      dc:date , dct:date ;
                    rdfs:label              "creation date"@en ;
                    dct:domainIncludes  aowm:Distribution ,
                                            aowm:CatalogRecord ,
                                            aowm:Catalog ;
                    rdfs:range              rdfs:Literal ; 
                    dct:description     "dct:date : A point or period of time associated with an event in the lifecycle of the resource. dct:created : Date of creation of the resource. dct:issued Date of formal issuance (e.g., publication) of the resource. PROV: Generation is the completion of production of a new entity by an activity. This entity did not exist before generation and becomes available for usage after this generation. PAV: The date this resource was authored. PAV: The date this resource was contributed to. PAV: The date of creation of the resource representation. DOAP: Date when something was created, in YYYY-MM-DD form. e.g. 2004-04-05. SCHEMA: The date on which the CreativeWork was created or the item was added to a DataFeed. DOAP: Date when something was created, in YYYY-MM-DD form. e.g. 2004-04-05."@en ;
                    rdfs:isDefinedBy        <http://purl.org/dc/terms/> ;
                    dct:issued          "2000-07-11"^^xsd:date ; 
                    owl:equivalentProperty  omv:creationDate ,
                                            dct:issued ,
                                            pav:authoredOn ,
                                            pav:contributedOn ,
                                            pav:createdOn ,
                                            schema:dateCreated ,
                                            doap:created ,
                                            oboinowl:date ,
                                            oboinowl:hasDate ,
                                            prov:generatedAtTime ,
                                            <http://www.isibang.ac.in/ns/mod/1.1/creationDate> .
            

### http://purl.org/dc/terms/modified
dct:modified    rdf:type                rdf:Property ; 
                    rdfs:subPropertyOf      dc:date , dct:date ;
                    rdfs:label              "modification date"@en ;
                    dct:domainIncludes  aowm:Distribution					,
                                            aowm:CatalogRecord ,
                                            aowm:Catalog ;
                    rdfs:range              rdfs:Literal ; 
                    dct:description     "OMV: Date of the last modification made to the ontology. dct:Date on which the resource was changed. PAV: The date of the last update of the resource. An update is a change which did not warrant making a new resource related using pav:previousVersion, for instance correcting a spelling mistake. SCHEMA: The date on which the CreativeWork was most recently modified or when the item's entry was modified within a DataFeed."@en ;
                    rdfs:isDefinedBy        <http://purl.org/dc/terms/> ;
                    dct:issued          "2000-07-11"^^xsd:date ; 
                    owl:equivalentProperty  omv:modificationDate ,
                                            schema:dateModified ,
                                            pav:lastUpdateOn ,
                                            <http://www.isibang.ac.in/ns/mod/1.1/creationDate> .
            

### http://purl.org/dc/terms/valid
dct:valid       rdf:type                rdf:Property ; 
                    rdfs:subPropertyOf      dc:date , dct:date ;
                    rdfs:label              "validity date"@en ;
                    dct:domainIncludes  aowm:Distribution ;
                    rdfs:range              rdfs:Literal ; 
                    dct:description     "dct: Date (often a range) of validity of a resource. PROV: Invalidation is the start of the destruction, cessation, or expiry of an existing entity by an activity. The entity is no longer available for use (or further invalidation) after invalidation. Any generation or usage of an entity precedes its invalidation. SCHEMA: The end date and time of the item (in ISO 8601 date format)."@en ;
                    rdfs:isDefinedBy        <http://purl.org/dc/terms/> ;
                    dct:issued          "2000-07-11"^^xsd:date ; 
                    owl:equivalentProperty  schema:endDate ,
                                            prov:invalidatedAtTime .   

         
### http://purl.org/pav/curatedOn
pav:curatedOn       rdf:type                owl:DatatypeProperty ;
                    rdfs:subPropertyOf      pav:contributedOn ;
                    rdfs:label              "curation date"@en ;
                    dct:domainIncludes  aowm:Distribution ,
                                            aowm:CatalogRecord ,
                                            aowm:Catalog ;
                    rdfs:range              xsd:date ;
                    dct:description     "Curation date"@en ;
                    rdfs:isDefinedBy        <http://purl.org/pav/> ;
                    dct:issued          "2014-08-28"^^xsd:date .


### http://purl.org/dc/terms/dateSubmitted
dct:dateSubmitted
                    rdf:type                rdf:Property ; 
                    rdfs:subPropertyOf      dc:date , dct:date ;
                    rdfs:label              "submission date"@en ;
                    dct:domainIncludes  aowm:Distribution ,
                                            aowm:CatalogRecord ;
                    rdfs:range              rdfs:Literal ; 
                    dct:description     "dct: Date of submission of the resource. SCHEMA: Date of first broadcast/publication."@en ;
                    rdfs:isDefinedBy        <http://purl.org/dc/terms/> ;
                    dct:issued          "2002-07-13"^^xsd:date ; 
                    owl:equivalentProperty  schema:datePublished .    



####elements and relations####
### http://www.w3.org/2002/07/owl#imports
owl:imports         rdf:type                owl:OntologyProperty  ;
                    rdfs:label              "imports"@en ;
                    rdfs:domain             owl:Ontology ;
                    dct:domainIncludes  aowm:Distribution ;
                    rdfs:range              owl:Ontology ;
                    dct:description     "OWL: References another OWL ontology containing definitions, whose meaning is considered to be part of the meaning of the importing ontology. OMV: References another ontology metadata instance that describes an ontology containing definitions, whose meaning is considered to be part of the meaning of the ontology described by this ontology metadata instance. dct: A related resource that is required by the described resource to support its function, delivery, or coherence. VOAF: Indicates that the subject vocabulary extends the expressivity of the object vocabulary by declaring subsumption relationships, using object vocabulary class as domain or range of a subject vocabulary property, defining local restrictions etc . ADMS: An Asset that is contained in the Asset being described, e.g. when there are several vocabularies defined in a single document."@en ;  
                    rdfs:isDefinedBy        <http://www.w3.org/2002/07/owl#> ;
                    dct:issued          "2004-02-10"^^xsd:date ;
                    owl:equivalentProperty  omv:useImports ,
                                            dct:requires ,
                                            voaf:extends ,
                                            adms:includedAsset .

### http://purl.org/dc/terms/isPartOf
dct:isPartOf    rdf:type                rdf:Property ;
                    rdfs:subPropertyOf      dc:relation , dct:relation ;
                    rdfs:label              "is part of (view of)"@en ;
                    dct:domainIncludes  aowm:Ontology ,
                                            aowm:Catalog ;
                    dct:description     "dct: A related resource in which the described resource is physically or logically included. MOD: Shall be used to identify a subset or a view of an ontology. DOOR: An ontology is included in another if its model is contained in the one of the other ontology. SCHEMA: Indicates an item or CreativeWork that this item, or CreativeWork (in some sense), is part of."@en ;
                    rdfs:isDefinedBy        <http://purl.org/dc/terms/> ;
                    dct:issued          "2000-07-11"^^xsd:date ;
                    owl:equivalentProperty  door:includedIn ,
                                            void:subset , 
                                            schema:isPartOf ,
                                            <http://www.isibang.ac.in/ns/mod/1.1/module> .
            

### http://purl.org/dc/terms/hasPart
dct:hasPart     rdf:type                rdf:Property ;
                    rdfs:subPropertyOf      dc:relation , dct:relation ;
                    rdfs:label              "has part (has view)"@en ;
                    dct:domainIncludes  aowm:Ontology ,
                                            aowm:Catalog ;
                    dct:description     "dct: A related resource that is included either physically or logically in the described resource. SCHEMA: Indicates an item or CreativeWork that is part of this item, or CreativeWork (in some sense). ADMS: Links to a sample of an Asset (which is itself an Asset)."@en ;
                    rdfs:isDefinedBy        <http://purl.org/dc/terms/> ;
                    dct:issued          "2000-07-11"^^xsd:date ;
                    owl:equivalentProperty  schema:hasPart ,
                                            adms:sample , 
                                            oboinowl:hasSubset ;
                    pav:derivedFrom        <https://w3id.org/mod/1.0> .


### http://www.w3.org/ns/dcat#catalog
dcat:catalog        rdf:type                rdf:Property , owl:ObjectProperty ;
                    rdfs:subPropertyOf      dct:hasPart , rdfs:member ;
                    rdfs:label              "catalog"@en ;
                    rdfs:domain             dcat:Catalog ;
                    dct:domainIncludes  mod:SemanticArtefactCatalog ;
                    rdfs:range              dcat:Catalog ;
                    dct:description     "DCAT:A catalog whose contents are of interest in the context of this catalog. dct: A related resource that is included either physically or logically in the described resource. SCHEMA: Indicates an item or CreativeWork that is part of this item, or CreativeWork (in some sense). ADMS: Links to a sample of an Asset (which is itself an Asset)."@en ;
                    rdfs:isDefinedBy        <http://www.w3.org/TR/vocab-dcat/> ;
                    dct:issued          "2020-02-20"^^xsd:date ;
                    owl:equivalentProperty  dct:hasPart ,
                                            schema:hasPart ,
                                            adms:sample ;
                    pav:derivedFrom         <https://w3id.org/mod/3.2> ;
                    pav:importedOn          "2024-06-25"^^xsd:date .
            
 
### http://purl.org/dc/terms/relation
dct:relation    rdf:type                rdf:Property ;
                    rdfs:subPropertyOf      dc:relation ;
                    rdfs:label              "relation"@en ,
                                            "relation"@fr ;
                    dct:domainIncludes  aowm:Ontology ,
                                            aowm:Catalog ;
                    dct:description     "dct: A related resource."@en ;
                    rdfs:isDefinedBy        <http://purl.org/dc/terms/> ;
                    dct:issued          "2008-01-14"^^xsd:date .


### http://www.w3.org/ns/dcat#qualifiedRelation
dcat:qualifiedRelation
                    rdf:type                rdf:Property , owl:ObjectProperty ;
                    rdfs:subPropertyOf      prov:qualifiedInfluence ;
                    rdfs:label              "qualified relation"@en ;
                    rdfs:domain             dcat:Resource ;
                    dct:domainIncludes  aowm:Ontology ,
                                            aowm:Catalog ;
                    rdfs:range              dcat:Relationship ;
                    dct:description     "DCAT: Link to a description of a relationship with another resource. PROV: Influence is the capacity of an entity, activity, or agent to have an effect on the character, development, or behavior of another by means of usage, start, end, generation, invalidation, communication, derivation, attribution, association, or delegation."@en ;
                    rdfs:isDefinedBy        <http://www.w3.org/TR/vocab-dcat/> ;
                    dct:issued          "2020-02-20"^^xsd:date ;
                    owl:equivalentProperty  schema:hasPart .
      
   
### https://w3id.org/mod#semanticArtefactRelation
mod:semanticArtefactRelation 
                    rdf:type                owl:ObjectProperty ;
                    rdfs:subPropertyOf      dct:relation ;
                    rdfs:label              "generally related to"@en ;
                    rdfs:domain             mod:SemanticArtefact ;
					dct:domainIncludes  	aowm:Ontology ;
                    rdfs:range              mod:SemanticArtefact ;
                    dct:description     "MOD: A general property for semantic artefact relations. DOOR: An ontology is related to another if one of the DOOR relations is satisfied."@en ;
                    rdfs:isDefinedBy        <https://w3id.org/mod/2.0> ;
                    dct:issued          "2021-12-06"^^xsd:date ;
                    owl:equivalentProperty  door:ontologyRelatedTo .


### https://w3id.org/mod#specializes
mod:specializes     rdf:type                owl:ObjectProperty ;
                    rdfs:subPropertyOf      mod:semanticArtefactRelation ;
                    owl:inverseOf           mod:generalizes ;
                    rdfs:label              "specializes"@en ;
                    dct:description     "DOOR: Evolution which involves a change only at the syntactic level. PROV: An entity that is a specialization of another shares all aspects of the latter, and additionally presents more specific aspects of the same thing as the latter. VOAF:Indicates that the subject vocabulary defines some subclasses or subproperties of the object vocabulary, or local restrictions on those."@en ;
                    rdfs:isDefinedBy        <http://purl.org/vocommons/voaf> ;
                    dct:issued          "2013-05-23"^^xsd:date ;
                    owl:equivalentProperty  door:explanationEvolution ,
                                            voaf:specializes ,
                                            prov:specializationOf .
            

### https://w3id.org/mod#generalizes
mod:generalizes     rdf:type                owl:ObjectProperty ;
                    rdfs:subPropertyOf      mod:semanticArtefactRelation ;
                    owl:inverseOf           mod:specializes ;
                    rdfs:label              "generalizes"@en ;
                    dct:description     "VOAF: Indicates that the subject vocabulary generalizes by some superclasses or superproperties the object vocabulary. PROV: Inverse property of specializationOf."@en ;
                    rdfs:isDefinedBy        <http://purl.org/vocommons/voaf> ;
                    dct:issued          "2013-05-23"^^xsd:date ;
                    owl:equivalentProperty  voaf:generalizes ,
                                            prov:generalizationOf .
            

## https://w3id.org/mod#usedBy
mod:usedBy          rdf:type                owl:ObjectProperty ;
                    rdfs:subPropertyOf      mod:semanticArtefactRelation ;
                    owl:inverseOf           mod:reliesOn ;
                    rdfs:label              "used by"@en ;
                    dct:description     "VOAF: Indicates that the subject vocabulary is used by the object vocabulary. NKOS: Agent using the described KOS."@en ;
                    rdfs:isDefinedBy        <http://purl.org/vocommons/voaf> ;
                    dct:issued          "2013-05-23"^^xsd:date ;
                    owl:equivalentProperty  voaf:usedBy ,
                                            nkos:usedBy .


### https://w3id.org/mod#reliesOn
mod:reliesOn        rdf:type                owl:ObjectProperty ;
                    rdfs:subPropertyOf      mod:semanticArtefactRelation ;
                    owl:inverseOf           mod:usedBy ;
                    rdfs:label              "relies on or reuses"@en ;
                    dct:description     "MOD: A general property for different kind of case when a semantic resource relies or reuses another one. VOAF: Indicates that the subject vocabulary uses or extends some class or property of the object vocabulary. VOID: A vocabulary that is used in the dataset."@en ;
                    rdfs:isDefinedBy        <http://purl.org/vocommons/voaf> ;
                    dct:issued          "2013-05-24"^^xsd:date ;
                    owl:equivalentProperty  voaf:reliesOn ,
                                            void:vocabulary  .


### https://w3id.org/mod#similar
mod:similar     rdf:type                    owl:ObjectProperty ;
                    rdfs:subPropertyOf      mod:semanticArtefactRelation ;
                    rdfs:label              "similar to"@en ,
                                            "similaire "@fr ;
                    dct:description     "VOAF: Used to assert that two vocabularies are similar in scope and objectives, independently of the fact that they otherwise refer to each other. DOOR: Represents the meaning of 'how an ontology overlap/cover parts of the same area of interest of another ontology.'"@en ;
                    rdfs:isDefinedBy        <http://purl.org/vocommons/voaf> ;
                    dct:issued          "2013-05-23"^^xsd:date ;
                    owl:equivalentProperty  <http://kannel.open.ac.uk/ontology/similarTo> ,
                                            voaf:similar ;
                    pav:derivedFrom         <https://w3id.org/mod/1.4> ;
                    pav:importedOn          "2018-08-02"^^xsd:date ;
            
            #OPTIONAL STATEMENTS
                    skos:historyNote        "This property had been originally defined by VOAF metadata vocabulary. Now, it has been adopted and redefined in the MOD namespace."@en ;
                    prov:wasInfluencedBy    "MIRO guidelines: B.2",
                                            "FAIR principle: I2" .


###  https://w3id.org/mod#comesFromTheSameDomain
mod:comesFromTheSameDomain
                    rdf:type                owl:ObjectProperty , owl:SymmetricProperty , owl:TransitiveProperty ;
                    rdfs:subPropertyOf      mod:semanticArtefactRelation ;
                    rdfs:label              "comes from the same domain"@en ;
                    dct:description     "DOOR: If the two ontologies come from the same domain (without any other details)."@en ;
                    rdfs:isDefinedBy        <http://kannel.open.ac.uk/ontology> ;
                    dct:issued          "2009-10-06"^^xsd:date ;
                    owl:equivalentProperty  <http://kannel.open.ac.uk/ontology/comesFromTheSameDomain> .
             

## https://w3id.org/mod#hasEquivalencesWith
mod:hasEquivalencesWith
                    rdf:type                owl:ObjectProperty ;
                    rdfs:subPropertyOf      mod:reliesOn ;
                    rdfs:label              "has equivalences with"@en ;
                    dct:description     "VOAF: Indicates that the subject vocabulary declares some equivalent classes or properties with the object vocabulary. DOOR: Links two ontologies if there exists an alignment which covers a substantial part of the vocabulary (i.e., a proportion greater than a threshold). NKOS: A related resource with which the described resource is aligned."@en ;
                    rdfs:isDefinedBy        <http://purl.org/vocommons/voaf> ;
                    dct:issued          "2013-05-23"^^xsd:date ;
                    owl:equivalentProperty  door:isAlignedTo ,
                                            voaf:hasEquivalencesWith ,
                                            nkos:alignedWith .


### http://www.w3.org/2002/07/owl#backwardCompatibleWith
owl:backwardCompatibleWith
                    rdf:type                owl:AnnotationProperty, owl:OntologyProperty  ;
                    rdfs:label              "backward compatible"@en ;
                    rdfs:domain             owl:Ontology ;
                    dct:domainIncludes  aowm:Ontology ;
                    rdfs:range              owl:Ontology ; 
                    dct:description     "OWL: This identifies the specified ontology as a prior version of the containing ontology, and further indicates that it is backward compatible with it. OMV: The ontology metadata instance which describes an ontology that is a compatible prior version of the ontology described by this ontology metadata Instance. DOOR: The relation of being a compatible new version from owl."@en ;  
                    rdfs:isDefinedBy        <http://www.w3.org/2002/07/owl#> ;
                    dct:issued          "2004-02-10"^^xsd:date ;
                    owl:equivalentProperty  omv:isBackwardCompatibleWith ,
                                            door:backwardCompatibleWith .


### http://www.w3.org/2002/07/owl#incompatibleWith
owl:incompatibleWith
                    rdf:type                owl:AnnotationProperty, owl:OntologyProperty  ;
                    rdfs:label              "incompatible"@en ;
                    rdfs:domain             owl:Ontology ;
                    dct:domainIncludes  aowm:Ontology ;
                    rdfs:range              owl:Ontology ; 
                    dct:description     "OWL: This indicates that the containing ontology is a later version of the referenced ontology, but is not backward compatible with it. OMV: The described ontology is a later version of the ontology described by the metadata specified, but is not backward compatible with it. It can be used to explicitly state that ontology cannot upgrade to use the new version without checking whether changes are required. "@en ;  
                    rdfs:isDefinedBy        <http://www.w3.org/2002/07/owl#> ;
                    dct:issued          "2004-02-10"^^xsd:date ;
                    owl:equivalentProperty  omv:isIncompatibleWith ,
                                            door:owlIncompatibleWith .
            
###  https://w3id.org/mod#hasDisparateModelling
mod:hasDisparateModelling
                    rdf:type                owl:ObjectProperty ;
                    rdfs:subPropertyOf      mod:semanticArtefactRelation ;
                    rdfs:label              "disparate modelling with"@en ;
                    dct:description     "DOOR: Disagreements related to the conceptualization of the ontologies. Two ontologies are considered to have disparate modeling if they represent corresponding entities in different ways, e.g.  as an instance in one case and a class in the other."@en ;
                    rdfs:isDefinedBy        <http://kannel.open.ac.uk/ontology> ;
                    dct:issued          "2009-10-06"^^xsd:date ;
                    owl:equivalentProperty  <http://kannel.open.ac.uk/ontology/hasDisparateModelling> .


## https://w3id.org/mod#hasDisjunctionsWith
mod:hasDisjunctionsWith
                    rdf:type                owl:ObjectProperty ;
                    rdfs:subPropertyOf      mod:semanticArtefactRelation ;
                    rdfs:label              "has disjunctions with"@en ;
                    dct:description     "VOAF: Indicates that the subject vocabulary declares some disjunct classes with the object vocabulary."@en ;
                    rdfs:isDefinedBy        <http://purl.org/vocommons/voaf> ;
                    dct:issued          "2013-05-23"^^xsd:date ;
                    owl:equivalentProperty  voaf:hasDisjunctionsWith .


## http://schema.org/workTranslation
schema:workTranslation
                    rdf:type                rdf:Property ;
                    rdfs:label              "work translation"@en ;
                    dct:domainIncludes  aowm:Ontology ;
                    dct:rangeIncludes   aowm:Ontology ;
                    dct:description     "MOD: A pointer to the translated ontology(ies) for an existing ontology. SCHEMA: A work that is a translation of the content of this work. ADMS: Links Assets that are translations of each other."@en ;
                    rdfs:isDefinedBy        <http://schema.org/> ;
                    dct:issued          "2012-04-21"^^xsd:date ;
                    owl:equivalentProperty  adms:translation ,
                                            <http://www.isibang.ac.in/ns/mod/1.0/translation> .
    

## http://schema.org/translationOfWork
schema:translationOfWork
                    rdf:type                rdf:Property ;
                    rdfs:label              "translation of"@en ;
                    dct:domainIncludes  aowm:Ontology ;
                    dct:rangeIncludes   aowm:Ontology ;
                    dct:description     "SCHEMA: The work that this work has been translated from. ADMS: Links Assets that are translations of each other."@en ;
                    rdfs:isDefinedBy        <http://schema.org/> ;
                    dct:issued          "2012-04-21"^^xsd:date ;
                    owl:equivalentProperty  adms:translation  .
					
					
					
					
####content####
### http://rdfs.org/ns/void#uriRegexPattern
void:uriRegexPattern
                    rdf:type                rdf:Property ;
                    rdfs:label              "identifier pattern"@en ;
                    rdfs:domain             void:Dataset ;
                    dct:domainIncludes  aowm:Ontology ,
                                            aowm:Catalog ;
                    dct:description     "VOID: A regular expression that matches the URIs of a void:Dataset's entities. IDOT: Regular expression describing alphanumeric strings used to identify items (or records) in a dataset."@en ;
                    rdfs:isDefinedBy        <http://vocab.deri.ie/void> ;
                    dct:issued          "2010-01-26"^^xsd:date ;
                    owl:equivalentProperty  idot:identifierPattern .


### http://purl.org/vocab/vann/preferredNamespaceUri
vann:preferredNamespaceUri 
                    rdf:type                owl:AnnotationProperty ;
                    rdfs:label              "preferred namespace URI"@en ;
                    dct:domainIncludes  aowm:Ontology ,
                                            aowm:Catalog ;
                    dct:description     "VANN: The preferred namespace URI to use when using terms from this vocabulary in an XML document. VOID: A URI that is a common string prefix of all the entity URIs in a void:Dataset."@en ;
                    rdfs:isDefinedBy        <http://purl.org/vocab/vann/> ;
                    dct:issued          "2005-04-01"^^xsd:date ;
                    owl:equivalentProperty  void:uriSpace .
            

### http://purl.org/vocab/vann/preferredNamespacePrefix
vann:preferredNamespacePrefix
                    rdf:type                owl:AnnotationProperty ;
                    rdfs:label              "preferred namespace prefix"@en ;
                    dct:domainIncludes  aowm:Ontology ,
                                            aowm:Catalog ;
                    dct:description     "VANN: The preferred namespace prefix to use when using terms from this vocabulary in an XML document. IDOT: Short label that is commonly used to refer to the dataset. Often utilised to identify the dataset in IRIs for specific items (or records). This may also stand in place of the base IRI of the dataset (e.g. see http://prefix.cc)."@en ; 
                    rdfs:isDefinedBy        <http://purl.org/vocab/vann/> ;
                    dct:issued          "2005-04-01"^^xsd:date ;
                    owl:equivalentProperty  idot:preferredPrefix ,
                                            oboinowl:default-namespace ,
                                            oboinowl:hasDefaultNamespace .
        

### https://w3id.org/mod#obsoleteParent
mod:obsoleteParent
                    rdf:type                owl:DatatypeProperty ;
                    rdfs:label              "root of obsolete branch"@en ;
                    rdfs:domain             mod:SemanticArtefactDistribution ;
					dct:domainIncludes		aowm:Distribution ;
                    rdfs:range              xsd:anyURI ;
                    dct:description     "MOD: Property used to specify the root of an obsolete branch in the ontology."@en ;
                    rdfs:isDefinedBy        <https://w3id.org/mod> ;
                    dct:issued          "2018-08-02"^^xsd:date .


### http://rdfs.org/ns/void#exampleResource
void:exampleResource
                    rdf:type                rdf:Property ;
                    rdfs:label              "example de resource"@en ;
                    rdfs:domain             void:Dataset ;
                    dct:domainIncludes  aowm:Ontology ;
                    rdfs:range              rdfs:Resource ;
                    dct:description     "VOID: Example resource of dataset. IDOT: An example identifier used by one item (or record) from a dataset."@en ;
                    rdfs:isDefinedBy        <http://vocab.deri.ie/void> ;
                    dct:issued          "2010-01-26"^^xsd:date ;
                    owl:equivalentProperty  idot:exampleIdentifier .


### http://xmlns.com/foaf/0.1/primaryTopic
foaf:primaryTopic   rdf:type                owl:ObjectProperty , owl:FunctionalProperty ;
                    rdfs:label              "key classes"@en ;
                    rdfs:domain             foaf:Document ;
                    dct:domainIncludes  aowm:Ontology ;
                    rdfs:range              owl:Thing ;
                    dct:description     "primary topic"@en ;
                    rdfs:isDefinedBy        <http://xmlns.com/foaf/0.1/> ;
                    dct:issued          "2014-01-14"^^xsd:date ;
                    owl:equivalentProperty  omv:keyClasses ,
                                            schema:mainEntity .


### https://w3id.org/mod#metadataVoc
mod:metadataVoc     rdf:type                owl:ObjectProperty ;
                    rdfs:label              "metadata vocabulary used"@en ;
                    rdfs:domain             mod:SemanticArtefactDistribution ,
                                            mod:SemanticArtefactCatalog ;
					dct:domainIncludes		aowm:Distribution,
											aowm:Catalog ;
                    rdfs:range              xsd:anyURI  ;
                    dct:description     "VOAF: Indicates that the subject vocabulary uses the object vocabulary in metadata at vocabulary or element level. SCHEMA: Indicates (by URL or string) a particular version of a schema used in some CreativeWork. MOD: A vocabulary(ies) that is used and/or referred to create the current ontology."@en ;    
                    rdfs:isDefinedBy        <http://purl.org/vocommons/voaf> ;
                    dct:issued          "2013-05-23"^^xsd:date ;
                    owl:equivalentProperty  voaf:metadataVoc ,
                                            schema:schemaVersion ,
                                            <http://www.isibang.ac.in/ns/mod/1.0/vocabularyUsed> .


### http://rdfs.org/ns/void#rootResource
void:rootResource   rdf:type                rdf:Property ;
                    rdfs:label              "root resource"@en ;
                    rdfs:domain             void:Dataset ;
                    dct:domainIncludes  aowm:Ontology ;
                    rdfs:range              rdfs:Resource ;
                    dct:description     "VOID: A top concept or entry point for a void:Dataset that is structured in a tree-like fashion. All resources in a dataset can be reached by following links from its root resources in a small number of steps. MOD: This property is to provide the root class(es) of an ontology. This is automatically populated by taking the direct subclasses of owl:Thing. If the ontology is also defined as a unique skos:ConceptScheme, then this property should become equivalent of skos:hasTopConcept. SKOS: The property skos:hasTopConcept is, by convention, used to link a concept scheme to the SKOS concept(s) which are topmost in the hierarchical relations for that scheme."@en ;
                    rdfs:isDefinedBy        <http://vocab.deri.ie/void> ;
                    dct:issued          "2010-01-26"^^xsd:date ;
                    owl:equivalentProperty  skos:hasTopConcept ,
                                            <http://www.isibang.ac.in/ns/mod/1.0/rootClasses> .


### http://rdfs.org/ns/void#classPartition
void:classPartition
                    rdf:type                rdf:Property ;
                    rdfs:label              "class partition"@en ;
                    rdfs:domain             void:Dataset ;
                    dct:domainIncludes  aowm:Ontology ;
                    rdfs:range              void:Dataset ;
                    dct:description     "VOID: A subset of a void:Dataset that contains only the entities of a certain rdfs:Class."@en ;
                    rdfs:isDefinedBy        <http://vocab.deri.ie/void> ;
                    dct:issued          "2010-01-26"^^xsd:date .


### http://rdfs.org/ns/void#propertyPartition
void:propertyPartition
                    rdf:type                rdf:Property ;
                    rdfs:label              "property partition"@en ;
                    rdfs:domain             void:Dataset ;
                    dct:domainIncludes  aowm:Ontology ;
                    rdfs:range              void:Dataset ;
                    dct:description     "VOID: A subset of a void:Dataset that contains only the triples of a certain rdf:Property."@en ;
                    rdfs:isDefinedBy        <http://vocab.deri.ie/void> ;
                    dct:issued          "2010-01-26"^^xsd:date .


### http://www.w3.org/ns/dcat#dataset
dcat:dataset        rdf:type                rdf:Property , owl:ObjectProperty ;
                    rdfs:subPropertyOf      dct:hasPart , rdfs:member ;
                    rdfs:label              "dataset"@en ;
                    rdfs:domain             dcat:Catalog ;
                    dct:domainIncludes  aowm:Catalog ;
                    rdfs:range              dcat:Dataset ;
                    dct:description     "DCAT: A collection of data that is listed in the catalog."@en ;
                    rdfs:isDefinedBy        <http://www.w3.org/TR/vocab-dcat/> ;
                    dct:issued          "2014-01-16"^^xsd:date .


### http://www.w3.org/ns/dcat#service
dcat:service        rdf:type                rdf:Property , owl:ObjectProperty ;
                    rdfs:subPropertyOf      dct:hasPart , rdfs:member ;
                    rdfs:label              "service"@en ;
                    rdfs:domain             dcat:Catalog ;
                    dct:domainIncludes  aowm:Catalog ;
                    rdfs:range              dcat:DataService ;
                    dct:description     "DCAT: A site or end-point that is listed in the catalog."@en ;
                    rdfs:isDefinedBy        <http://www.w3.org/TR/vocab-dcat/> ;
                    dct:issued          "2020-02-04"^^xsd:date .


### http://www.w3.org/ns/dcat#record
dcat:record        rdf:type                rdf:Property , owl:ObjectProperty ;
                    rdfs:label              "catalog record"@en ;
                    rdfs:domain             dcat:Catalog ;
                    dct:domainIncludes  aowm:Catalog ;
                    rdfs:range              dcat:CatalogRecord ;
                    dct:description     "DCAT: A record describing the registration of a single dataset or data service that is part of the catalog."@en ;
                    rdfs:isDefinedBy        <http://www.w3.org/TR/vocab-dcat/> ;
                    dct:issued          "2014-01-16"^^xsd:date .


### http://www.w3.org/ns/dcat#themeTaxonomy
dcat:themeTaxonomy  rdf:type                rdf:Property , owl:ObjectProperty ;
                    rdfs:label              "theme taxonomy"@en ;
                    rdfs:domain             dcat:Catalog ;
                    dct:domainIncludes  aowm:Catalog ;
                    rdfs:range              rdfs:Resource ;
                    dct:description     "DCAT: A knowledge organization system (KOS) used to classify catalog's datasets and services."@en ;
                    rdfs:isDefinedBy        <http://www.w3.org/TR/vocab-dcat/> ;
                    dct:issued          "2014-01-16"^^xsd:date .
  

####distribution####
### http://www.w3.org/ns/dcat#distribution
dcat:distribution   rdf:type                rdf:Property , owl:ObjectProperty ;
                    rdfs:subPropertyOf      dct:relation ;
                    rdfs:label              "distribution"@en ;
                    rdfs:domain             dcat:Dataset ;
                    dct:domainIncludes  aowm:Catalog ;
                    rdfs:range              dcat:Distribution ;
                    dct:description     "DCAT: An available distribution of the dataset."@en ;
                    rdfs:isDefinedBy        <http://www.w3.org/TR/vocab-dcat/> ;
                    dct:issued          "2014-01-16"^^xsd:date ;
                    pav:derivedFrom         <https://w3id.org/mod/3.2> ;
                    pav:importedOn          "2024-06-25"^^xsd:date .
  
aowm:hasDistribution
	a owl:ObjectProperty ;
	rdfs:domain aowm:Ontology ;
	rdfs:range aowm:Distribution ;
	rdfs:label "Distribution"@en ;
	dct:description "Distribution of an ontology."@en ;
    rdfs:isDefinedBy <http://dqm.faw.jku.at/ontologies/aowm> .

####versioning and evolution#####
### http://www.w3.org/2002/07/owl#PriorVersion
owl:PriorVersion    rdf:type                owl:AnnotationProperty, owl:OntologyProperty  ;
                    rdfs:label              "prior version"@en ;
                    rdfs:domain             owl:Ontology ;
                    dct:domainIncludes  	aowm:Ontology ;
                    rdfs:range              owl:Ontology ; 
                    dct:description     "OWL:  This identifies the specified ontology as a prior version of the containing ontology. OMV: Contains a reference to another ontology metadata instance. dct: A related resource of which the described resource is a version, edition, or adaptation. PROV: A revision is a derivation for which the resulting entity is a revised version of some original. The implication here is that the resulting entity contains substantial content from the original. DOOR: Prior version relation from OWL. ADMS: A link to the previous version of the Asset."@en ;  
                    rdfs:isDefinedBy        <http://www.w3.org/2002/07/owl#> ;
                    dct:issued          "2004-02-10"^^xsd:date ;
                    owl:equivalentProperty  omv:hasPriorVersion ,
                                            dct:isVersionOf ,
                                            prov:wasRevisionOf ,
                                            door:priorVersion ,
                                            adms:prev .
											
### http://purl.org/dc/terms/hasVersion
dct:hasVersion  rdf:type                rdf:Property ;
                    rdfs:label              "has version"@en ;
                    dct:domainIncludes  aowm:Ontology ;
					dct:rangeIncludes	aowm:Version ;
                    dct:description     "dct: a related resource that is a version, edition, or adaptation of the described resource. MOD: A related ontology that is a version, edition, or adaptation of the described ontology. PAV: This resource has a more specific, versioned resource."@en ;
                    rdfs:isDefinedBy        <http://purl.org/dc/terms/> ;
                    dct:issued          "2000-07-11"^^xsd:date ;
                    owl:equivalentProperty  pav:hasVersion , 
                                            <http://www.isibang.ac.in/ns/mod/1.2/version> .
					
### https://vocab.org/vann/changes
vann:changes        rdf:type                owl:AnnotationProperty ;
                    rdfs:subPropertyOf      rdfs:seeAlso ;
                    rdfs:label              "changes"@en ;
                    dct:domainIncludes  aowm:Ontology ,
                                            aowm:Catalog ;
                    dct:description     "VANN: A reference to a resource that describes changes between this version of a vocabulary and the previous."@en ;
                    rdfs:isDefinedBy        <http://purl.org/vocab/vann/> ;
                    dct:issued          "2005-04-01"^^xsd:date .
					
### http://www.w3.org/2002/07/owl#versionIRI
owl:versionIRI      rdf:type                owl:OntologyProperty ;
                    rdfs:label              "version IRI"@en ;
                    rdfs:domain             owl:Ontology ;
                    dct:domainIncludes  aowm:Ontology ;
                    rdfs:range              owl:Ontology ;
                    dct:rangeIncludes   	aowm:Ontology ;
                    dct:description     "OWL: The property that identifies the version IRI of an ontology."@en ;  
                    rdfs:isDefinedBy        <http://www.w3.org/2002/07/owl#> ;
                    dct:issued          "2004-02-10"^^xsd:date .
		
### http://www.w3.org/2002/07/owl#versionInfo		
owl:versionInfo  
	rdf:type owl:AnnotationProperty ;
    rdfs:label "version information"@en ;
    dct:domainIncludes  
		aowm:Ontology ,
		aowm:Catalog ;
	rdfs:domain rdfs:Resource ;
	rdfs:range xsd:string ;
    dct:description     "MOD: The version of the released ontology. OMV: The version information of the ontology. OWL: The annotation property that provides version information for an ontology or another OWL construct. PAV: The version number of a resource. This is a freetext string, typical values are '1.5' or '21'. DOAP: A project release."@en ;  
    rdfs:isDefinedBy <http://www.w3.org/2002/07/owl#> ;
    dct:issued          "2004-02-10"^^xsd:date ;
    owl:equivalentProperty  
		skos:notation ,
        schema:identifier .
		
### https://w3id.org/mod#status
mod:status          rdf:type                owl:DatatypeProperty ;
                    rdfs:label              "status"@en ;
                    rdfs:domain             mod:SemanticArtefact ,
                                            mod:SemanticArtefactCatalog ;
					dct:domainIncludes	aowm:Ontology ,
											aowm:Catalog ;
                    rdfs:range              xsd:string ;
                    dct:description     "OMV: It specifies the tracking information for the contents of the ontology. Pre-defined values. IDOT: State of a resource (physical location providing access to data or information about the identified entity). This is should be based on a recent manual or automatic check of the resource. Possible values are: 'up', 'down', 'probably up', 'obsolete resource', 'restricted access' and 'unknown'. SCHEMA: The status of a creative work in terms of its stage in a lifecycle. Example terms include Incomplete, Draft, Published, Obsolete. Some organizations define a set of terms for the stages of their publication lifecycle."@en ;
                    rdfs:isDefinedBy        <http://omv.ontoware.org/2005/05/ontology> ;
                    dct:issued          "2009-12-24"^^xsd:date ;
                    owl:equivalentProperty  idot:state ,
                                            adms:adms-status ,
                                            schema:creativeWorkStatus .
		
aowm:madeChange
    a owl:ObjectProperty ;
    rdfs:label "person who is responsible for the change"@en ;
    rdfs:domain aowm:Ontology ;
    rdfs:range 	aowm:Agent ;
    dct:description "Specifies the person which changed something in this version. Annotate with vann:changes"@en ;#
	dct:issued          "2026-01-30"^^xsd:date ;
    rdfs:isDefinedBy <http://dqm.faw.jku.at/ontologies/aowm> .
	
####quality and maturity####
aowm:degreeOfMaturity
	a owl:DatatypeProperty ;
	rdfs:label "Degree of Maturity"@en ;
	rdfs:domain aowm:Ontology ;
    rdfs:range 	aowm:DegreeOfMaturity ;
	dct:description: "Degree of maturity of an ontology"@en ;
	dct:issued          "2026-01-30"^^xsd:date ;
	rdfs:isDefinedBy <http://dqm.faw.jku.at/ontologies/aowm> .
	
aowm:coverageRatio
	a owl:DatatypeProperty ;
	rdfs:label "Coverage Ratio"@en ;
	rdfs:domain aowm:Ontology ;
	rdfs:range xsd:string ;
	dct:description: "Coverage ratio of an ontology"@en ;
	dct:issued          "2026-01-30"^^xsd:date ;
	rdfs:isDefinedBy <http://dqm.faw.jku.at/ontologies/aowm> .
	
aowm:restrictions
	a owl:DatatypeProperty ;
	rdfs:label "Restrictions"@en ;
	rdfs:domain aowm:Ontology ;
	rdfs:range xsd:string ;
	dct:description: "Restrictions of an ontology"@en ;
	dct:issued          "2026-01-30"^^xsd:date ;
	rdfs:isDefinedBy <http://dqm.faw.jku.at/ontologies/aowm> .
	
####technical representation####
aowm:serializations
	a owl:ObjectProperty ;
	rdfs:label "Serializations"@en ;
	rdfs:domain aowm:Ontology ,
				aowm:Distribution ;
	rdfs:range 	aowm:SerializationFormat ;
	dct:description: "Serializations of an ontology"@en ;
	dct:issued          "2026-01-30"^^xsd:date ;
	rdfs:isDefinedBy <http://dqm.faw.jku.at/ontologies/aowm> .
	
####maintenance and lifecycle####
### http://www.w3.org/2002/07/owl#deprecated
owl:deprecated     rdf:type                owl:AnnotationProperty ; 
                   rdfs:label              "deprecated"@en ;
                   rdfs:domain             rdfs:Resource ;
                   dct:domainIncludes  aowm:Ontology ,
                                           aowm:Distribution ,
                                           aowm:Catalog ;
                   rdfs:range              rdfs:Resource ;
                   dct:description     "OWL: The annotation property that indicates that a given entity has been deprecated. IDOT: Indicates if the current dataset is obsolete (not provided any more to the public community). Value can either be 'true' or 'false' (xsd:boolean). The statement is usually omitted if 'false'."@en ;
                   rdfs:isDefinedBy        <http://www.w3.org/2002/07/owl#> ;
                   dct:issued          "2004-02-10"^^xsd:date ;
                   owl:equivalentProperty  idot:obsolete ,
                                           <http://www.isibang.ac.in/ns/mod/1.1/deprecated> .
										   
aowm:supportPeriod
	a owl:DatatypeProperty ;
	rdfs:label "Support Period"@en ;
	rdfs:domain aowm:Ontology ;
	rdfs:range xsd:string ;
	dct:description "Planned period of support for an ontology"@en ;
	dct:issued          "2026-01-30"^^xsd:date ;
	rdfs:isDefinedBy <http://dqm.faw.jku.at/ontologies/aowm> .

aowm:successorArtifacts
	a owl:DatatypeProperty ;
	rdfs:label "Successor Artifacts"@en ;
	rdfs:domain aowm:Ontology ;
	rdfs:range xsd:anyURI ;
	dct:description: "Successor artifacts an ontology"@en ;
	dct:issued "2026-01-30"^^xsd:date ;
	rdfs:isDefinedBy <http://dqm.faw.jku.at/ontologies/aowm> .
										   
####object descriptions#####
### https://w3id.org/mod#prefLabelProperty
mod:prefLabelProperty
					rdf:type                owl:DatatypeProperty ;
                    rdfs:label              "object preferred label property"@en;
					rdfs:domain             mod:SemanticArtefactDistribution ;
                    rdfs:range              xsd:anyURI ;
					dct:domainIncludes 		aowm:Distribution ;
                    dct:description     "MOD: Property used to specify object's preferred label."@en ;
                    rdfs:isDefinedBy        <https://w3id.org/mod> ;
                    dct:issued          "2018-08-02"^^xsd:date ;
                    pav:derivedFrom         <https://w3id.org/mod/1.4> .
					
### https://w3id.org/mod#synonymProperty		
mod:synonymProperty rdf:type                owl:DatatypeProperty ;
                    rdfs:label              "object synonym property"@en ;
                    rdfs:domain             mod:SemanticArtefactDistribution ;
                    rdfs:range              xsd:anyURI ;
					dct:domainIncludes 		aowm:Distribution ;
                    dct:description     "MOD: Property used to specify object's synonym."@en ;
                    rdfs:isDefinedBy        <https://w3id.org/mod> ;
                    dct:issued          "2018-08-02"^^xsd:date ;
                    owl:equivalentProperty  oboinowl:hasSynonymType ,
                                            oboinowl:synonymtypedef ;
                    pav:derivedFrom         <https://w3id.org/mod/1.4> .
										
### https://w3id.org/mod#definitionProperty
mod:definitionProperty  
                    rdf:type                owl:DatatypeProperty ;
                    rdfs:label              "object definition property"@en ;
                    rdfs:domain             mod:SemanticArtefactDistribution ;
                    rdfs:range              xsd:anyURI ;
					dct:domainIncludes 		aowm:Distribution ;
                    dct:description     "MOD: Property used to specify object's definition."@en ;
                    rdfs:isDefinedBy        <https://w3id.org/mod> ;
                    dct:issued          "2018-08-02"^^xsd:date ;
                    pav:derivedFrom         <https://w3id.org/mod/1.4> .
					
### https://w3id.org/mod#authorProperty
mod:authorProperty  rdf:type                owl:DatatypeProperty ;
                    rdfs:label              "object author property"@en ;
                    rdfs:domain             mod:SemanticArtefactDistribution ;
                    rdfs:range              xsd:anyURI ;
					dct:domainIncludes 		aowm:Distribution ;
                    dct:description     "MOD: Property used to specify object's author."@en ;
                    rdfs:isDefinedBy        <https://w3id.org/mod> ;
                    dct:issued          "2018-08-02"^^xsd:date ;
                    pav:derivedFrom         <https://w3id.org/mod/1.4> .
											
### https://w3id.org/mod#obsoleteProperty
mod:obsoleteProperty
                    rdf:type               owl:DatatypeProperty ;
                    rdfs:label              "object obsolete property"@en ;
                    rdfs:domain             mod:SemanticArtefactDistribution ;
                    rdfs:range              xsd:anyURI ;
					dct:domainIncludes 		aowm:Distribution ;
                    dct:description     "MOD: Property used to specify obsolete object."@en ;
                    rdfs:isDefinedBy        <https://w3id.org/mod> ;
                    dct:issued          "2018-08-02"^^xsd:date ;
                    pav:derivedFrom         <https://w3id.org/mod/1.4> .

### https://w3id.org/mod#createdProperty
mod:createdProperty rdf:type               owl:DatatypeProperty ;
                    rdfs:label              "object creation date property"@en ;
                    rdfs:domain             mod:SemanticArtefactDistribution ;
                    rdfs:range              xsd:anyURI ;
					dct:domainIncludes 		aowm:Distribution ;
                    dct:description     "MOD: Property used to specify the date of creation of a class or another object in the ontology."@en ;
                    rdfs:isDefinedBy        <https://w3id.org/mod> ;
                    dct:issued          "2024-05-30"^^xsd:date ;
                    pav:derivedFrom         <https://w3id.org/mod/3.1> .

### https://w3id.org/mod#modifiedProperty
mod:modifiedProperty
                    rdf:type               owl:DatatypeProperty ;
                    rdfs:label              "object modification date property"@en ;
                    rdfs:domain             mod:SemanticArtefactDistribution ;
                    rdfs:range              xsd:anyURI ;
					dct:domainIncludes 		aowm:Distribution ;
                    dct:description     "MOD: Property used to specify the date of modification of a class or another object in the ontology."@en ;
                    rdfs:isDefinedBy        <https://w3id.org/mod> ;
                    dct:issued          "2024-05-30"^^xsd:date ;
                    pav:derivedFrom         <https://w3id.org/mod/3.1> .


### https://w3id.org/mod#hierarchyProperty
mod:hierarchyProperty
                    rdf:type                owl:DatatypeProperty ;
                    rdfs:label              "transitive hierarchy property"@en ;
                    rdfs:domain             mod:SemanticArtefactDistribution ;
                    rdfs:range              xsd:anyURI ;
					dct:domainIncludes 		aowm:Distribution ;
                    dct:description     "MOD: Property used to specify the hierarchy (e.g. rdfs:subClassOf or skos:broader)."@en ;
                    rdfs:isDefinedBy        <https://w3id.org/mod> ;
                    dct:issued          "2018-08-02"^^xsd:date ;
                    pav:derivedFrom         <https://w3id.org/mod/1.4> .
					
aowm:authorContact
	a owl:DatatypeProperty ;
	rdfs:label "Contact Data Author"@en ;
	rdfs:domain aowm:Ontology ;
	rdfs:range xsd:string ;
	dct:description: "Data in order to contact the author of an ontoloy, e.g. phone number or email."@en ;
	dct:issued          "2026-02-01"^^xsd:date ;
	rdfs:isDefinedBy <http://dqm.faw.jku.at/ontologies/aowm> .

####Methodology and provenance####
### https://w3id.org/mod#conformsToKnowledgeRepresentationParadigm
mod:conformsToKnowledgeRepresentationParadigm
                    rdf:type                owl:ObjectProperty ;
                    rdfs:label              "knowledge representation paradigm"@en ;
                    rdfs:domain             mod:SemanticArtefactDistribution ;
					dct:domainIncludes		aowm:Distribution ;
                    rdfs:range              mod:KnowledgeRepresentationParadigm ;
                    dct:description     "MOD: A representation formalism that is followed to describe knowledge in an ontology. Examples include description logics, first order logic, etc. OMV: Information about the paradigm model used to create the ontology. dct: An established standard to which the described resource conforms."@en ;
                    rdfs:isDefinedBy        <http://omv.ontoware.org/2005/05/ontology> ;
                    dct:issued          "2009-12-24"^^xsd:date ;
                    owl:equivalentProperty  omv:conformsToKnowledgeRepresentationParadigm , 
                                            dct:conformsTo ,
                                            <http://www.isibang.ac.in/ns/mod/1.0/knowledgeRepresentationFormalism> .


### http://purl.org/dc/terms/conformsTo
dct:conformsTo  rdf:type                rdf:Property ;
                    rdfs:subPropertyOf      dc:relation, dct:relation ;
                    rdfs:label              "conforms to"@en ;
                    dct:domainIncludes  aowm:Catalog ;
                    dct:description     "dct: An established standard to which the described resource conforms."@en ;
                    rdfs:isDefinedBy        <http://purl.org/dc/terms/> ;
                    dct:issued          "2001-05-21"^^xsd:date .      



### https://w3id.org/mod#usedEngineeringMethodology
mod:usedEngineeringMethodology
                    rdf:type                owl:ObjectProperty ;
                    rdfs:label              "engineering methodology"@en ;
                    rdfs:domain             mod:SemanticArtefactDistribution;
					dct:domainIncludes		aowm:Distribution ;
                    rdfs:range              mod:EngineeringMethodology ;
                    dct:description     "MOD: A methodology following which an ontology is created. OMV: Information about the method model used to create the ontology."@en ;
                    rdfs:isDefinedBy        <http://omv.ontoware.org/2005/05/ontology> ;
                    dct:issued          "2009-12-24"^^xsd:date ;
                    owl:equivalentProperty  adms:representationTechnique ,
                                            schema:publishingPrinciples ,
                                            <http://www.isibang.ac.in/ns/mod/1.0/methodologyUsed> .


### http://purl.org/pav/createdWith
pav:createdWith     rdf:type                owl:ObjectProperty ;
                    rdfs:subPropertyOf      prov:wasAttributedTo ;
                    rdfs:label              "created with"@en ;
                    dct:domainIncludes   aowm:Ontology ,
                                            aowm:Catalog ;
                    dct:description     "PAV: The software/tool used by the creator (pav:createdBy) when making the digital resource, for instance a word processor or an annotation tool. MOD: The tool used for the creation of an ontology. OMV: Information about the tool used to create the ontology."@en ;
                    rdfs:isDefinedBy        <http://purl.org/pav/> ;
                    dct:issued          "2014-08-28"^^xsd:date ;
                    owl:equivalentProperty  omv:usedOntologyEngineeringTool ,
                                            oboinowl:auto-generated-by , 
                                            <http://www.isibang.ac.in/ns/mod/1.0/toolUsed> .
        

### http://purl.org/dc/terms/accrualMethod
dct:accrualMethod
                    rdf:type                rdf:Property ;
                    rdfs:label              "accrual method"@en ;
                    rdfs:domain             <http://purl.org/dc/dcmitype/Collection> ;
                    dct:domainIncludes   aowm:Ontology ,
                                            aowm:Catalog ;
                    dct:description     "dct: The method by which items are added to a collection. Recommended practice is to use a value from the Collection Description Accrual Method Vocabulary."@en ;
                    rdfs:isDefinedBy        <http://purl.org/dc/terms/> ;
                    dct:issued          "2005-06-13"^^xsd:date .


### http://purl.org/dc/terms/accrualPeriodicity
dct:accrualPeriodicity
                    rdf:type                rdf:Property ;
                    rdfs:label              "accrual periodicity"@en ;
                    rdfs:domain             <http://purl.org/dc/dcmitype/Collection> ;
                    dct:domainIncludes  aowm:Ontology ,
                                            aowm:Catalog ;
                    dct:description     "dct: The frequency with which items are added to a collection. Recommended practice is to use a value from the Collection Description Frequency Vocabulary."@en ;
                    rdfs:isDefinedBy        <http://purl.org/dc/terms/> ;
                    dct:issued          "2005-06-13"^^xsd:date .
                  
    
### http://purl.org/dc/terms/accrualPolicy
dct:accrualPolicy
                    rdf:type                rdf:Property ;
                    rdfs:label              "accrual policy"@en ;
                    rdfs:domain             <http://purl.org/dc/dcmitype/Collection> ;
                    dct:domainIncludes  aowm:Ontology ,
                                            aowm:Catalog ;
                    dct:description     "dct: The policy governing the addition of items to a collection. Recommended practice is to use a value from the Collection Description Accrual Policy Vocabulary."@en ;
                    rdfs:isDefinedBy        <http://purl.org/dc/terms/> ;
                    dct:issued          "2005-06-13"^^xsd:date .
        

### https://w3id.org/mod#competencyQuestion
mod:competencyQuestion 
                    rdf:type                owl:DatatypeProperty ;
                    rdfs:label              "competency question"@en ;
                    rdfs:domain             mod:SemanticArtefact ;
					dct:domainIncludes		aowm:Ontology ;
                    rdfs:range              xsd:string ;
                    dct:description     "MOD: A set of questions made to build an ontology at the design time."@en ;
                    rdfs:isDefinedBy        <https://w3id.org/mod> ;
                    dct:issued          "2015-08-05"^^xsd:date .


### https://w3id.org/mod#sampleQueries
mod:sampleQueries   rdf:type                owl:DatatypeProperty ;
                    rdfs:label              "sample queries"@en ;
                    rdfs:domain             mod:SemanticArtefactDistribution ,
                                            mod:SemanticArtefactCatalog ;
					dct:domainIncludes	aowm:Distribution,
											aowm:Catalog ;
                    rdfs:range              mod:string ;
                    dct:description     "MOD: A set of queries (may be SPARQL, DL Queries) that are provided along with an ontology."@en ;    
                    rdfs:isDefinedBy        <https://w3id.org/mod> ;
                    dct:issued          "2015-08-05"^^xsd:date .


### http://www.w3.org/ns/prov#wasGeneratedBy
prov:wasGeneratedBy rdf:type                owl:ObjectProperty ;
                    rdfs:subPropertyOf      prov:wasInfluencedBy ;
                    rdfs:label              "was generated by"@en ;
                    rdfs:domain             prov:Entity ;
                    dct:domainIncludes  aowm:Ontology ,
                                            aowm:Catalog ;
                    rdfs:range              prov:Activity ;
                    dct:description     "PROV: Generation is the completion of production of a new entity by an activity. This entity did not exist before generation and becomes available for usage after this generation. DCAT: An activity that generated, or provides the business context for, the creation of the dataset."@en ;
                    rdfs:isDefinedBy        <http://www.w3.org/ns/prov-o#> ;
                    dct:issued          "2013-04-30"^^xsd:date .


### http://www.w3.org/ns/prov#wasinvalidatedBy
prov:wasinvalidatedBy
                    rdf:type                owl:ObjectProperty ;
                    rdfs:subPropertyOf      prov:wasInfluencedBy ;
                    rdfs:label              "was invalidated by"@en ;
                    rdfs:domain             prov:Entity ;
                    dct:domainIncludes  aowm:Ontology ;
                    rdfs:range              prov:Activity ;
                    dct:description     "PROV: Invalidation is the start of the destruction, cessation, or expiry of an existing entity by an activity. The entity is no longer available for use (or further invalidation) after invalidation. Any generation or usage of an entity precedes its invalidation."@en ;
                    rdfs:isDefinedBy        <http://www.w3.org/ns/prov-o#> ;
                    dct:issued          "2013-04-30"^^xsd:date .


### https://w3id.org/mod#fairAssessment
mod:fairAssessment  rdf:type                owl:DatatypeProperty ;
                    rdfs:label              "FAIR assessment"@en ;
                    rdfs:domain             mod:SemanticArtefactDistribution ;
					dct:domainIncludes		aowm:Distribution ;
                    rdfs:range              mod:FairAssessment ;
                    dct:description     "MOD: A FAIRness assessment result produced by a known or identified FAIRness assessment method or tool. It can be either a simple number or a structured result document explaining the assessment."@en ;
                    rdfs:isDefinedBy        <https://w3id.org/mod> ;
                    dct:issued          "2024-05-30"^^xsd:date .         
				
####metadata about metadata####
aowm:metadataCreationMethod
	a owl:DatatypeProperty ;
	rdfs:label "Creation Method"@en ;
	rdfs:domain aowm:Ontology,
				aowm:Catalog ;
	rdfs:range 	aowm:MetadataCreationMethod ;
	dct:description: "Creation method of metadata - manual, automatic, semi-automatic"@en ;
	dct:issued          "2026-01-30"^^xsd:date ;
	rdfs:isDefinedBy <http://dqm.faw.jku.at/ontologies/aowm> .
	
aowm:metadataSource
	a owl:DatatypeProperty ;
	rdfs:label "Metadata Source"@en ;
	rdfs:domain aowm:Ontology,
				aowm:Catalog ;
	rdfs:range xsd:anyURI ;
	dct:description: "Source of metadata, e.g. repository, person,..."@en ;
	dct:issued          "2026-01-30"^^xsd:date ;
	rdfs:isDefinedBy <http://dqm.faw.jku.at/ontologies/aowm> .
	
aowm:metadataGeneratedBy
	a owl:DatatypeProperty ;
	rdfs:label "Metadata Generated By"@en ;
	rdfs:domain aowm:Ontology,
				aowm:Catalog ;
	rdfs:range xsd:string ;
	dct:description: "System or software which created the metadata"@en ;
	dct:issued          "2026-01-30"^^xsd:date ;
	rdfs:isDefinedBy <http://dqm.faw.jku.at/ontologies/aowm> .
	
aowm:metadataDerivedFrom
	a owl:DatatypeProperty ;
	rdfs:label "Metadata Derived From"@en ;
	rdfs:domain aowm:Ontology,
				aowm:Catalog ;
	rdfs:range xsd:anyURI ;
	dct:description: "Other metadata or artifacts, from which this metadata were derived"@en ;
	dct:issued          "2026-01-30"^^xsd:date ;
	rdfs:isDefinedBy <http://dqm.faw.jku.at/ontologies/aowm> .
	
aowm:metadataCreationDate
	a owl:DatatypeProperty ;
	rdfs:label "Metadata Creation Date"@en ;
	rdfs:domain aowm:Ontology,
				aowm:Catalog ;
	rdfs:range xsd:dateTime ;
	dct:description: "Time when metadata was initial created."@en ;
	dct:issued          "2026-01-30"^^xsd:date ;
	rdfs:isDefinedBy <http://dqm.faw.jku.at/ontologies/aowm> .

aowm:metadataCreator
	a owl:ObjectProperty ;
	rdfs:label "Metadata Creator"@en ;
	rdfs:domain aowm:Ontology,
				aowm:Catalog ;
	rdfs:range 	aowm:Agent ;
	dct:description "Agent (person or organization) that created the metadata."@en ;
	dct:issued "2026-01-30"^^xsd:date ;
	rdfs:isDefinedBy <http://dqm.faw.jku.at/ontologies/aowm> ;
	owl:equivalentProperty dct:creator, pav:authoredBy .

aowm:metadataMaintainer
	a owl:ObjectProperty ;
	rdfs:label "Metadata Maintainer"@en ;
	rdfs:domain aowm:Ontology,
				aowm:Catalog ;
	rdfs:range 	aowm:Agent ;
	dct:description "Person or organization responsible for maintaining the metadata."@en ;
	dct:issued "2026-01-30"^^xsd:date ;
	rdfs:isDefinedBy <http://dqm.faw.jku.at/ontologies/aowm> .
	
aowm:metadataCuratorRole
	a owl:ObjectProperty ;
	rdfs:label "Metadata Curator Role"@en ;
	rdfs:domain aowm:Ontology,
				aowm:Catalog ;
	rdfs:range 	aowm:Role ;
	dct:description "Role of the agent involved in metadata curation (e.g., editor, reviewer, validator)."@en ;
	dct:issued "2026-01-30"^^xsd:date ;
	rdfs:isDefinedBy <http://dqm.faw.jku.at/ontologies/aowm> .
	
aowm:metadataTrustLevel
	a owl:DatatypeProperty ;
	rdfs:label "Metadata Trust Level"@en ;
	rdfs:domain aowm:Ontology,
				aowm:Catalog ;
	rdfs:range xsd:string ;
	dct:description "Indicates the assessed trust level of the metadata."@en ;
	dct:issued "2026-01-30"^^xsd:date ;
	rdfs:isDefinedBy <http://dqm.faw.jku.at/ontologies/aowm> .
	
aowm:metadataCompleteness
	a owl:DatatypeProperty ;
	rdfs:label "Metadata Completeness"@en ;
	rdfs:domain aowm:Ontology,
				aowm:Catalog ;
	rdfs:range xsd:string ;
	dct:description "Indicates the degree of completeness of the metadata."@en ;
	dct:issued "2026-01-30"^^xsd:date ;
	rdfs:isDefinedBy <http://dqm.faw.jku.at/ontologies/aowm> .
	
aowm:metadataValidationStatus
	a owl:DatatypeProperty ;
	rdfs:label "Metadata Validation Status"@en ;
	rdfs:domain aowm:Ontology,
				aowm:Catalog ;
	rdfs:range xsd:string ;
	dct:description "Describes whether and how the metadata has been validated."@en ;
	dct:issued "2026-01-30"^^xsd:date ;
	rdfs:isDefinedBy <http://dqm.faw.jku.at/ontologies/aowm> .
	
aowm:metadataLastModified
	a owl:DatatypeProperty ;
	rdfs:label "Metadata Last Modified"@en ;
	rdfs:domain aowm:Ontology,
				aowm:Catalog ;
	rdfs:range xsd:date ;
	dct:description "Date of the last modification of the metadata."@en ;
	dct:issued "2026-01-30"^^xsd:date ;
	rdfs:isDefinedBy <http://dqm.faw.jku.at/ontologies/aowm> .
	
aowm:metadataUpdateFrequency
	a owl:DatatypeProperty ;
	rdfs:label "Metadata Update Frequency"@en ;
	rdfs:domain aowm:Ontology,
				aowm:Catalog ;
	rdfs:range xsd:string ;
	dct:description "Expected frequency at which the metadata is updated."@en ;
	dct:issued "2026-01-30"^^xsd:date ;
	rdfs:isDefinedBy <http://dqm.faw.jku.at/ontologies/aowm> .
	
aowm:metadataAutomationLevel
	a owl:DatatypeProperty ;
	rdfs:label "Metadata Automation Level"@en ;
	rdfs:domain aowm:Ontology,
				aowm:Catalog ;
	rdfs:range xsd:string ;
	dct:description "Indicates the degree of automation involved in creating the metadata."@en ;
	dct:issued "2026-01-30"^^xsd:date ;
	rdfs:isDefinedBy <http://dqm.faw.jku.at/ontologies/aowm> .
	
aowm:metadataVersion
	a owl:DatatypeProperty ;
	rdfs:label "Metadata Version"@en ;
	rdfs:domain aowm:Ontology,
				aowm:Catalog ;
	rdfs:range xsd:string ;
	dct:description "Version identifier of the metadata."@en ;
	dct:issued "2026-01-30"^^xsd:date ;
	rdfs:isDefinedBy <http://dqm.faw.jku.at/ontologies/aowm> .
	
aowm:metadataScope
	a owl:DatatypeProperty ;
	rdfs:label "Metadata Scope"@en ;
	rdfs:domain aowm:Ontology,
				aowm:Catalog ;
	rdfs:range xsd:string ;
	dct:description "Scope in which the metadata is applicable."@en ;
	dct:issued "2026-01-30"^^xsd:date ;
	rdfs:isDefinedBy <http://dqm.faw.jku.at/ontologies/aowm> .
	
aowm:metadataIntendedAudience
	a owl:DatatypeProperty ;
	rdfs:label "Metadata Intended Audience"@en ;
	rdfs:domain aowm:Ontology,
				aowm:Catalog ;
	rdfs:range xsd:string ;
	dct:description "Intended audience for which the metadata is provided."@en ;
	dct:issued "2026-01-30"^^xsd:date ;
	rdfs:isDefinedBy <http://dqm.faw.jku.at/ontologies/aowm> .

aowm:metadataUsageContext
	a owl:DatatypeProperty ;
	rdfs:label "Metadata Usage Context"@en ;
	rdfs:domain aowm:Ontology,
				aowm:Catalog ;
	rdfs:range xsd:string ;
	dct:description "Context in which the metadata is intended to be used."@en ;
	dct:issued "2026-01-30"^^xsd:date ;
	rdfs:isDefinedBy <http://dqm.faw.jku.at/ontologies/aowm> .
	
####Miscellaneous####
aowm:hasOntology
	a owl:ObjectProperty ;
	rdfs:domain aowm:Record ;
	rdfs:range aowm:Ontology ;
	rdfs:label "Has Ontology"@en ;
	dct:description "Ontology belonging to a catalog record."@en ;
	dct:issued "2026-01-30"^^xsd:date ;
    rdfs:isDefinedBy <http://dqm.faw.jku.at/ontologies/aowm> .
	
aowm:hasRecord
	a owl:ObjectProperty ;
	rdfs:domain aowm:Catalog ;
	rdfs:range aowm:CatalogRecord ;
	rdfs:label "Has Record"@en ;
	dct:description "Record belonging to a catalog."@en ;
	dct:issued "2026-01-30"^^xsd:date ;
    rdfs:isDefinedBy <http://dqm.faw.jku.at/ontologies/aowm> .
	
aowm:hasAgent a owl:ObjectProperty ;
	rdfs:label "Has Agent"@en ;
    rdfs:domain aowm:Ontology ;
    rdfs:range aowm:Agent ;
	dct:description "Agent belonging to a ontology/catalog."@en ;
	dct:issued "2026-01-30"^^xsd:date ;
	rdfs:isDefinedBy <http://dqm.faw.jku.at/ontologies/aowm> .

aowm:hasRole a owl:ObjectProperty ;
	rdfs:label "Has Role"@en ;
    rdfs:domain aowm:Ontology, aowm:Catalog ;
    rdfs:range aowm:Role ;
	dct:description "Role belonging to a ontology/catalog."@en ;
	dct:issued "2026-01-30"^^xsd:date ;
	rdfs:isDefinedBy <http://dqm.faw.jku.at/ontologies/aowm> .
	
aowm:hasVersion
    a owl:ObjectProperty ;
    rdfs:domain aowm:Ontology, aowm:CatalogRecord ;
    rdfs:range aowm:Version ;
    rdfs:label "Has Version"@en ;
    dct:description "Links an ontology or catalog record to a specific version."@en ;
	dct:issued "2026-01-30"^^xsd:date ;
	owl:equivalentProperty dct:hasVersion ;
	rdfs:isDefinedBy <http://dqm.faw.jku.at/ontologies/aowm> .
	
aowm:availableAs
    a owl:ObjectProperty ;
    rdfs:domain aowm:Ontology, aowm:Distribution ;
    rdfs:range aowm:SerializationFormat ;
    rdfs:label "Available As"@en ;
    dct:description "Indicates that the ontology or distribution is available in this serialization format."@en ;
	dct:issued "2026-01-30"^^xsd:date ;
    rdfs:isDefinedBy <http://dqm.faw.jku.at/ontologies/aowm> .
	
aowm:assumesRole
    a owl:ObjectProperty ;
    rdfs:domain aowm:Agent ;
    rdfs:range aowm:Role ;
    rdfs:label "Assumes Role"@en ;
    dct:description "An agent assumes a certain role in relation to an ontology or catalog."@en ;
	dct:issued "2026-01-30"^^xsd:date ;
    rdfs:isDefinedBy <http://dqm.faw.jku.at/ontologies/aowm> .
	
aowm:expressedInDSL
	a owl:DatatypeProperty ;
	rdfs:label "Used DSL"@en ;
	rdfs:domain aowm:Ontology ;
	rdfs:range 	xsd:string ;
	dct:description: "Reference to the DSL in which something is formulated."@en ;
	dct:issued  "2026-02-01"^^xsd:date ;
	rdfs:isDefinedBy <http://dqm.faw.jku.at/ontologies/aowm> .